<?xml version="1.0"?>
<rdf:RDF xmlns="http://purls.helmholtz-metadaten.de/cmso/"
     xml:base="http://purls.helmholtz-metadaten.de/cmso/"
     xmlns:dc="http://purl.org/dc/elements/1.1/"
     xmlns:owl="http://www.w3.org/2002/07/owl#"
     xmlns:rdf="http://www.w3.org/1999/02/22-rdf-syntax-ns#"
     xmlns:xml="http://www.w3.org/XML/1998/namespace"
     xmlns:xsd="http://www.w3.org/2001/XMLSchema#"
     xmlns:rdfs="http://www.w3.org/2000/01/rdf-schema#"
     xmlns:skos="http://www.w3.org/2004/02/skos/core#"
     xmlns:terms="http://purl.org/dc/terms/">
    <owl:Ontology rdf:about="http://purls.helmholtz-metadaten.de/cmso/">
        <terms:contributor>https://orcid.org/0000-0001-9560-4728</terms:contributor>
        <terms:contributor>https://orcid.org/0000-0002-5149-603X</terms:contributor>
        <terms:contributor>https://orcid.org/0000-0002-6776-1213</terms:contributor>
        <terms:contributor>https://orcid.org/0000-0003-0698-4891</terms:contributor>
        <terms:creator>https://orcid.org/0000-0001-7564-7990</terms:creator>
        <terms:description>CMSO is an ontology that aims to describe computational materials science samples (or structures), including crystalline defects.</terms:description>
        <terms:title>Computational Material Sample Ontology (CMSO)</terms:title>
    </owl:Ontology>
    


    <!-- 
    ///////////////////////////////////////////////////////////////////////////////////////
    //
    // Annotation properties
    //
    ///////////////////////////////////////////////////////////////////////////////////////
     -->

    


    <!-- http://purl.org/dc/elements/1.1/contributor -->

    <owl:AnnotationProperty rdf:about="http://purl.org/dc/elements/1.1/contributor"/>
    


    <!-- http://purl.org/dc/elements/1.1/creator -->

    <owl:AnnotationProperty rdf:about="http://purl.org/dc/elements/1.1/creator"/>
    


    <!-- http://purl.org/dc/elements/1.1/description -->

    <owl:AnnotationProperty rdf:about="http://purl.org/dc/elements/1.1/description"/>
    


    <!-- http://purl.org/dc/elements/1.1/title -->

    <owl:AnnotationProperty rdf:about="http://purl.org/dc/elements/1.1/title"/>
    


    <!-- http://purl.org/dc/terms/abstract -->

    <owl:AnnotationProperty rdf:about="http://purl.org/dc/terms/abstract">
        <rdfs:subPropertyOf rdf:resource="http://purl.org/dc/terms/description"/>
    </owl:AnnotationProperty>
    


    <!-- http://purl.org/dc/terms/alternative -->

    <owl:AnnotationProperty rdf:about="http://purl.org/dc/terms/alternative">
        <rdfs:subPropertyOf rdf:resource="http://purl.org/dc/terms/title"/>
    </owl:AnnotationProperty>
    


    <!-- http://purl.org/dc/terms/contributor -->

    <owl:AnnotationProperty rdf:about="http://purl.org/dc/terms/contributor">
        <rdfs:comment xml:lang="en-us">Examples of a Contributor include a person, an organization, or a service. Typically, the name of a Contributor should be used to indicate the entity.</rdfs:comment>
        <rdfs:label xml:lang="en-us">Contributor</rdfs:label>
        <skos:definition xml:lang="en-us">An entity responsible for making contributions to the resource.</skos:definition>
        <rdfs:subPropertyOf rdf:resource="http://purl.org/dc/elements/1.1/contributor"/>
    </owl:AnnotationProperty>
    


    <!-- http://purl.org/dc/terms/creator -->

    <owl:AnnotationProperty rdf:about="http://purl.org/dc/terms/creator">
        <rdfs:comment xml:lang="en-us">Examples of a Creator include a person, an organization, or a service. Typically, the name of a Creator should be used to indicate the entity.</rdfs:comment>
        <rdfs:label xml:lang="en-us">Creator</rdfs:label>
        <skos:definition xml:lang="en-us">An entity primarily responsible for making the resource.</skos:definition>
        <rdfs:subPropertyOf rdf:resource="http://purl.org/dc/elements/1.1/creator"/>
        <rdfs:subPropertyOf rdf:resource="http://purl.org/dc/terms/contributor"/>
        <rdfs:range rdf:resource="http://purl.org/dc/terms/Agent"/>
    </owl:AnnotationProperty>
    


    <!-- http://purl.org/dc/terms/description -->

    <owl:AnnotationProperty rdf:about="http://purl.org/dc/terms/description">
        <rdfs:comment xml:lang="en-us">Description may include but is not limited to: an abstract, a table of contents, a graphical representation, or a free-text account of the resource.</rdfs:comment>
        <rdfs:label xml:lang="en-us">Description</rdfs:label>
        <skos:definition xml:lang="en-us">An account of the resource.</skos:definition>
        <rdfs:subPropertyOf rdf:resource="http://purl.org/dc/elements/1.1/description"/>
    </owl:AnnotationProperty>
    


    <!-- http://purl.org/dc/terms/tableOfContents -->

    <owl:AnnotationProperty rdf:about="http://purl.org/dc/terms/tableOfContents">
        <rdfs:subPropertyOf rdf:resource="http://purl.org/dc/terms/description"/>
    </owl:AnnotationProperty>
    


    <!-- http://purl.org/dc/terms/title -->

    <owl:AnnotationProperty rdf:about="http://purl.org/dc/terms/title">
        <rdfs:label xml:lang="en-us">Title</rdfs:label>
        <skos:definition xml:lang="en-us">A name given to the resource.</skos:definition>
        <skos:note xml:lang="en-us">In current practice, this term is used primarily with literal values; however, there are important uses with non-literal values as well. As of December 2007, the DCMI Usage Board is leaving this range unspecified pending an investigation of options.</skos:note>
        <rdfs:subPropertyOf rdf:resource="http://purl.org/dc/elements/1.1/title"/>
    </owl:AnnotationProperty>
    


    <!-- http://www.w3.org/2004/02/skos/core#altLabel -->

    <owl:AnnotationProperty rdf:about="http://www.w3.org/2004/02/skos/core#altLabel">
        <rdfs:comment xml:lang="en">The range of skos:altLabel is the class of RDF plain literals.</rdfs:comment>
        <rdfs:comment xml:lang="en">skos:prefLabel, skos:altLabel and skos:hiddenLabel are pairwise disjoint properties.</rdfs:comment>
        <rdfs:isDefinedBy rdf:resource="http://www.w3.org/2004/02/skos/core"/>
        <rdfs:label xml:lang="en">alternative label</rdfs:label>
        <skos:definition xml:lang="en">An alternative lexical label for a resource.</skos:definition>
        <skos:example xml:lang="en">Acronyms, abbreviations, spelling variants, and irregular plural/singular forms may be included among the alternative labels for a concept. Mis-spelled terms are normally included as hidden labels (see skos:hiddenLabel).</skos:example>
        <rdfs:subPropertyOf rdf:resource="http://www.w3.org/2000/01/rdf-schema#label"/>
    </owl:AnnotationProperty>
    


    <!-- http://www.w3.org/2004/02/skos/core#definition -->

    <owl:AnnotationProperty rdf:about="http://www.w3.org/2004/02/skos/core#definition">
        <rdfs:isDefinedBy rdf:resource="http://www.w3.org/2004/02/skos/core"/>
        <rdfs:label xml:lang="en">definition</rdfs:label>
        <skos:definition xml:lang="en">A statement or formal explanation of the meaning of a concept.</skos:definition>
        <rdfs:subPropertyOf rdf:resource="http://www.w3.org/2004/02/skos/core#note"/>
    </owl:AnnotationProperty>
    


    <!-- http://www.w3.org/2004/02/skos/core#example -->

    <owl:AnnotationProperty rdf:about="http://www.w3.org/2004/02/skos/core#example">
        <rdfs:isDefinedBy rdf:resource="http://www.w3.org/2004/02/skos/core"/>
        <rdfs:label xml:lang="en">example</rdfs:label>
        <skos:definition xml:lang="en">An example of the use of a concept.</skos:definition>
        <rdfs:subPropertyOf rdf:resource="http://www.w3.org/2004/02/skos/core#note"/>
    </owl:AnnotationProperty>
    


    <!-- http://www.w3.org/2004/02/skos/core#note -->

    <owl:AnnotationProperty rdf:about="http://www.w3.org/2004/02/skos/core#note">
        <skos:definition xml:lang="en">A general note, for any purpose.</skos:definition>
    </owl:AnnotationProperty>
    


    <!-- http://www.w3.org/2004/02/skos/core#prefLabel -->

    <owl:AnnotationProperty rdf:about="http://www.w3.org/2004/02/skos/core#prefLabel">
        <rdfs:comment xml:lang="en">A resource has no more than one value of skos:prefLabel per language tag, and no more than one value of skos:prefLabel without language tag.</rdfs:comment>
        <rdfs:comment xml:lang="en">The range of skos:prefLabel is the class of RDF plain literals.</rdfs:comment>
        <rdfs:comment xml:lang="en">skos:prefLabel, skos:altLabel and skos:hiddenLabel are pairwise
      disjoint properties.</rdfs:comment>
        <rdfs:isDefinedBy rdf:resource="http://www.w3.org/2004/02/skos/core"/>
        <rdfs:label xml:lang="en">preferred label</rdfs:label>
        <skos:definition xml:lang="en">The preferred lexical label for a resource, in a given language.</skos:definition>
        <rdfs:subPropertyOf rdf:resource="http://www.w3.org/2000/01/rdf-schema#label"/>
    </owl:AnnotationProperty>
    


    <!-- 
    ///////////////////////////////////////////////////////////////////////////////////////
    //
    // Datatypes
    //
    ///////////////////////////////////////////////////////////////////////////////////////
     -->

    


    <!-- http://qudt.org/schema/qudt/LatexString -->

    <rdfs:Datatype rdf:about="http://qudt.org/schema/qudt/LatexString"/>
    


    <!-- 
    ///////////////////////////////////////////////////////////////////////////////////////
    //
    // Object Properties
    //
    ///////////////////////////////////////////////////////////////////////////////////////
     -->

    


    <!-- http://purls.helmholtz-metadaten.de/cmso/hasAngle -->

    <owl:ObjectProperty rdf:about="http://purls.helmholtz-metadaten.de/cmso/hasAngle">
        <rdfs:domain>
            <owl:Class>
                <owl:unionOf rdf:parseType="Collection">
                    <rdf:Description rdf:about="http://purls.helmholtz-metadaten.de/cmso/SimulationCell"/>
                    <rdf:Description rdf:about="http://purls.helmholtz-metadaten.de/cmso/UnitCell"/>
                </owl:unionOf>
            </owl:Class>
        </rdfs:domain>
        <rdfs:range rdf:resource="http://purls.helmholtz-metadaten.de/cmso/Angle"/>
        <rdfs:label>has angle</rdfs:label>
        <skos:definition>The relation between a simulation or unit cell and its angle.</skos:definition>
    </owl:ObjectProperty>
    


    <!-- http://purls.helmholtz-metadaten.de/cmso/hasAtom -->

    <owl:ObjectProperty rdf:about="http://purls.helmholtz-metadaten.de/cmso/hasAtom">
        <rdfs:domain rdf:resource="http://purls.helmholtz-metadaten.de/cmso/AtomicScaleSample"/>
        <rdfs:range rdf:resource="http://purls.helmholtz-metadaten.de/cmso/Atom"/>
        <rdfs:label>has atom</rdfs:label>
        <skos:definition>The relation between an atomic scale sample and the atoms it contains.</skos:definition>
    </owl:ObjectProperty>
    


    <!-- http://purls.helmholtz-metadaten.de/cmso/hasBasis -->

    <owl:ObjectProperty rdf:about="http://purls.helmholtz-metadaten.de/cmso/hasBasis">
        <rdfs:domain rdf:resource="http://purls.helmholtz-metadaten.de/cmso/UnitCell"/>
        <rdfs:range rdf:resource="http://purls.helmholtz-metadaten.de/cmso/Basis"/>
        <rdfs:label>has basis</rdfs:label>
        <skos:definition>The relation between a unit cell and the basis of the crystal structure.</skos:definition>
    </owl:ObjectProperty>
    


    <!-- http://purls.helmholtz-metadaten.de/cmso/hasCalculatedProperty -->

    <owl:ObjectProperty rdf:about="http://purls.helmholtz-metadaten.de/cmso/hasCalculatedProperty">
        <owl:inverseOf rdf:resource="http://purls.helmholtz-metadaten.de/cmso/isCalculatedPropertyOf"/>
        <rdfs:domain rdf:resource="http://purls.helmholtz-metadaten.de/cmso/ComputationalSample"/>
        <rdfs:range rdf:resource="http://purls.helmholtz-metadaten.de/cmso/CalculatedProperty"/>
        <rdfs:label>has calculated property</rdfs:label>
        <skos:definition>The relation between a computational sample and the calculated property.</skos:definition>
    </owl:ObjectProperty>
    


    <!-- http://purls.helmholtz-metadaten.de/cmso/hasDefect -->

    <owl:ObjectProperty rdf:about="http://purls.helmholtz-metadaten.de/cmso/hasDefect">
        <owl:inverseOf rdf:resource="http://purls.helmholtz-metadaten.de/cmso/isDefectOf"/>
        <rdfs:domain rdf:resource="http://purls.helmholtz-metadaten.de/cmso/CrystallineMaterial"/>
        <rdfs:range rdf:resource="http://purls.helmholtz-metadaten.de/cmso/CrystalDefect"/>
        <rdfs:label>has defect</rdfs:label>
        <skos:definition>The relation between  a crystalline material and the crystal defects it contains.</skos:definition>
    </owl:ObjectProperty>
    


    <!-- http://purls.helmholtz-metadaten.de/cmso/hasElement -->

    <owl:ObjectProperty rdf:about="http://purls.helmholtz-metadaten.de/cmso/hasElement">
        <rdfs:domain rdf:resource="http://purls.helmholtz-metadaten.de/cmso/ChemicalSpecies"/>
        <rdfs:range rdf:resource="http://purls.helmholtz-metadaten.de/cmso/ChemicalElement"/>
        <rdfs:label>has element</rdfs:label>
        <skos:definition>The relation between an atom and its chemical element.</skos:definition>
    </owl:ObjectProperty>
    


    <!-- http://purls.helmholtz-metadaten.de/cmso/hasLatticeParameter -->

    <owl:ObjectProperty rdf:about="http://purls.helmholtz-metadaten.de/cmso/hasLatticeParameter">
        <rdfs:domain rdf:resource="http://purls.helmholtz-metadaten.de/cmso/UnitCell"/>
        <rdfs:range rdf:resource="http://purls.helmholtz-metadaten.de/cmso/LatticeParameter"/>
        <rdfs:label>has lattice parameter</rdfs:label>
        <skos:definition>The relation between a unit cell and its lattice parameters.</skos:definition>
    </owl:ObjectProperty>
    


    <!-- http://purls.helmholtz-metadaten.de/cmso/hasLength -->

    <owl:ObjectProperty rdf:about="http://purls.helmholtz-metadaten.de/cmso/hasLength">
        <rdfs:domain rdf:resource="http://purls.helmholtz-metadaten.de/cmso/SimulationCell"/>
        <rdfs:range rdf:resource="http://purls.helmholtz-metadaten.de/cmso/Length"/>
        <rdfs:label>has length</rdfs:label>
        <skos:definition>The relation between a simulation cell and its length.</skos:definition>
    </owl:ObjectProperty>
    


    <!-- http://purls.helmholtz-metadaten.de/cmso/hasMaterial -->

    <owl:ObjectProperty rdf:about="http://purls.helmholtz-metadaten.de/cmso/hasMaterial">
        <owl:inverseOf rdf:resource="http://purls.helmholtz-metadaten.de/cmso/isMaterialOf"/>
        <rdfs:domain rdf:resource="http://purls.helmholtz-metadaten.de/cmso/ComputationalSample"/>
        <rdfs:range rdf:resource="http://purls.helmholtz-metadaten.de/cmso/Material"/>
        <rdfs:label>has material</rdfs:label>
        <skos:definition>The relation between a computational sample and the material it represents.</skos:definition>
    </owl:ObjectProperty>
    


    <!-- http://purls.helmholtz-metadaten.de/cmso/hasPositionVector -->

    <owl:ObjectProperty rdf:about="http://purls.helmholtz-metadaten.de/cmso/hasPositionVector">
        <rdfs:subPropertyOf rdf:resource="http://purls.helmholtz-metadaten.de/cmso/hasVector"/>
        <rdfs:domain>
            <owl:Class>
                <owl:unionOf rdf:parseType="Collection">
                    <rdf:Description rdf:about="http://purls.helmholtz-metadaten.de/cmso/Atom"/>
                    <rdf:Description rdf:about="http://purls.helmholtz-metadaten.de/cmso/Basis"/>
                </owl:unionOf>
            </owl:Class>
        </rdfs:domain>
        <rdfs:range rdf:resource="http://purls.helmholtz-metadaten.de/cmso/PositionVector"/>
        <rdfs:label>has position vector</rdfs:label>
        <skos:definition>The relation between an atom or basis and its position vector.</skos:definition>
    </owl:ObjectProperty>
    


    <!-- http://purls.helmholtz-metadaten.de/cmso/hasSimulationCell -->

    <owl:ObjectProperty rdf:about="http://purls.helmholtz-metadaten.de/cmso/hasSimulationCell">
        <rdfs:domain rdf:resource="http://purls.helmholtz-metadaten.de/cmso/AtomicScaleSample"/>
        <rdfs:range rdf:resource="http://purls.helmholtz-metadaten.de/cmso/SimulationCell"/>
        <rdfs:label>has simulation cell</rdfs:label>
        <skos:definition>The relation between an atomic scale sample and the simulation cell.</skos:definition>
    </owl:ObjectProperty>
    


    <!-- http://purls.helmholtz-metadaten.de/cmso/hasSpaceGroup -->

    <owl:ObjectProperty rdf:about="http://purls.helmholtz-metadaten.de/cmso/hasSpaceGroup">
        <rdfs:domain rdf:resource="http://purls.helmholtz-metadaten.de/cmso/CrystalStructure"/>
        <rdfs:range rdf:resource="http://purls.helmholtz-metadaten.de/cmso/SpaceGroup"/>
        <rdfs:label>has space group</rdfs:label>
        <skos:definition>The relation between a crystal structure and the space group that describes the symmetry.</skos:definition>
    </owl:ObjectProperty>
    


    <!-- http://purls.helmholtz-metadaten.de/cmso/hasSpecies -->

    <owl:ObjectProperty rdf:about="http://purls.helmholtz-metadaten.de/cmso/hasSpecies">
        <rdfs:domain rdf:resource="http://purls.helmholtz-metadaten.de/cmso/Material"/>
        <rdfs:range rdf:resource="http://purls.helmholtz-metadaten.de/cmso/ChemicalSpecies"/>
        <rdfs:label>has species</rdfs:label>
        <skos:definition>The relation between a material and the species that constitutes it.</skos:definition>
    </owl:ObjectProperty>
    


    <!-- http://purls.helmholtz-metadaten.de/cmso/hasStructure -->

    <owl:ObjectProperty rdf:about="http://purls.helmholtz-metadaten.de/cmso/hasStructure">
        <rdfs:domain rdf:resource="http://purls.helmholtz-metadaten.de/cmso/Material"/>
        <rdfs:range rdf:resource="http://purls.helmholtz-metadaten.de/cmso/Structure"/>
        <rdfs:label>has structure</rdfs:label>
        <skos:definition>The relation between a material and its structure.</skos:definition>
    </owl:ObjectProperty>
    


    <!-- http://purls.helmholtz-metadaten.de/cmso/hasUnit -->

    <owl:ObjectProperty rdf:about="http://purls.helmholtz-metadaten.de/cmso/hasUnit">
        <rdfs:domain>
            <owl:Class>
                <owl:unionOf rdf:parseType="Collection">
                    <rdf:Description rdf:about="http://purls.helmholtz-metadaten.de/cmso/Angle"/>
                    <rdf:Description rdf:about="http://purls.helmholtz-metadaten.de/cmso/CalculatedProperty"/>
                    <rdf:Description rdf:about="http://purls.helmholtz-metadaten.de/cmso/Length"/>
                    <rdf:Description rdf:about="http://purls.helmholtz-metadaten.de/cmso/Vector"/>
                </owl:unionOf>
            </owl:Class>
        </rdfs:domain>
        <rdfs:range rdf:resource="http://qudt.org/schema/qudt/Unit"/>
        <rdfs:label>has unit</rdfs:label>
        <skos:definition>A relation indicating the unit.</skos:definition>
    </owl:ObjectProperty>
    


    <!-- http://purls.helmholtz-metadaten.de/cmso/hasUnitCell -->

    <owl:ObjectProperty rdf:about="http://purls.helmholtz-metadaten.de/cmso/hasUnitCell">
        <rdfs:domain rdf:resource="http://purls.helmholtz-metadaten.de/cmso/CrystalStructure"/>
        <rdfs:range rdf:resource="http://purls.helmholtz-metadaten.de/cmso/UnitCell"/>
        <rdfs:label>has unit cell</rdfs:label>
        <skos:definition>The relation between a crystal structure and its unit cell.</skos:definition>
    </owl:ObjectProperty>
    


    <!-- http://purls.helmholtz-metadaten.de/cmso/hasVector -->

    <owl:ObjectProperty rdf:about="http://purls.helmholtz-metadaten.de/cmso/hasVector">
        <rdfs:domain>
            <owl:Class>
                <owl:unionOf rdf:parseType="Collection">
                    <rdf:Description rdf:about="http://purls.helmholtz-metadaten.de/cmso/SimulationCell"/>
                    <rdf:Description rdf:about="http://purls.helmholtz-metadaten.de/cmso/UnitCell"/>
                </owl:unionOf>
            </owl:Class>
        </rdfs:domain>
        <rdfs:range rdf:resource="http://purls.helmholtz-metadaten.de/cmso/Vector"/>
        <rdfs:label>has vector</rdfs:label>
        <skos:definition>The relation between a simulation or unit cell and its vectors.</skos:definition>
    </owl:ObjectProperty>
    


    <!-- http://purls.helmholtz-metadaten.de/cmso/isCalculatedPropertyOf -->

    <owl:ObjectProperty rdf:about="http://purls.helmholtz-metadaten.de/cmso/isCalculatedPropertyOf">
        <rdfs:label>is calculated property of</rdfs:label>
    </owl:ObjectProperty>
    


    <!-- http://purls.helmholtz-metadaten.de/cmso/isDefectOf -->

    <owl:ObjectProperty rdf:about="http://purls.helmholtz-metadaten.de/cmso/isDefectOf">
        <rdfs:label>is defect of</rdfs:label>
    </owl:ObjectProperty>
    


    <!-- http://purls.helmholtz-metadaten.de/cmso/isMaterialOf -->

    <owl:ObjectProperty rdf:about="http://purls.helmholtz-metadaten.de/cmso/isMaterialOf">
        <rdfs:label>is material of</rdfs:label>
    </owl:ObjectProperty>
    


    <!-- 
    ///////////////////////////////////////////////////////////////////////////////////////
    //
    // Data properties
    //
    ///////////////////////////////////////////////////////////////////////////////////////
     -->

    


    <!-- http://purls.helmholtz-metadaten.de/cmso/hasAltName -->

    <owl:DatatypeProperty rdf:about="http://purls.helmholtz-metadaten.de/cmso/hasAltName">
        <rdfs:subPropertyOf rdf:resource="http://purls.helmholtz-metadaten.de/cmso/hasName"/>
        <rdfs:domain rdf:resource="http://www.w3.org/2002/07/owl#Thing"/>
        <rdfs:range rdf:resource="http://www.w3.org/2001/XMLSchema#string"/>
        <rdfs:label>has alternative name</rdfs:label>
        <skos:definition>A data property linking an entity with alternative names.</skos:definition>
    </owl:DatatypeProperty>
    


    <!-- http://purls.helmholtz-metadaten.de/cmso/hasAngle_alpha -->

    <owl:DatatypeProperty rdf:about="http://purls.helmholtz-metadaten.de/cmso/hasAngle_alpha">
        <rdfs:domain rdf:resource="http://purls.helmholtz-metadaten.de/cmso/Angle"/>
        <rdfs:range rdf:resource="http://www.w3.org/2001/XMLSchema#float"/>
        <rdfs:label>has angle alpha</rdfs:label>
        <skos:definition>A data property linking the angle to the measurement in the x axis.</skos:definition>
    </owl:DatatypeProperty>
    


    <!-- http://purls.helmholtz-metadaten.de/cmso/hasAngle_beta -->

    <owl:DatatypeProperty rdf:about="http://purls.helmholtz-metadaten.de/cmso/hasAngle_beta">
        <rdfs:domain rdf:resource="http://purls.helmholtz-metadaten.de/cmso/Angle"/>
        <rdfs:range rdf:resource="http://www.w3.org/2001/XMLSchema#float"/>
        <rdfs:label>has angle beta</rdfs:label>
        <skos:definition>A data property linking the angle to the measurement in the y axis.</skos:definition>
    </owl:DatatypeProperty>
    


    <!-- http://purls.helmholtz-metadaten.de/cmso/hasAngle_gamma -->

    <owl:DatatypeProperty rdf:about="http://purls.helmholtz-metadaten.de/cmso/hasAngle_gamma">
        <rdfs:domain rdf:resource="http://purls.helmholtz-metadaten.de/cmso/Angle"/>
        <rdfs:range rdf:resource="http://www.w3.org/2001/XMLSchema#float"/>
        <rdfs:label>has angle gamma</rdfs:label>
        <skos:definition>A data property linking the angle to the measurement in the z axis.</skos:definition>
    </owl:DatatypeProperty>
    


    <!-- http://purls.helmholtz-metadaten.de/cmso/hasChemicalSymbol -->

    <owl:DatatypeProperty rdf:about="http://purls.helmholtz-metadaten.de/cmso/hasChemicalSymbol">
        <rdfs:subPropertyOf rdf:resource="http://purls.helmholtz-metadaten.de/cmso/hasSymbol"/>
        <rdfs:domain rdf:resource="http://purls.helmholtz-metadaten.de/cmso/ChemicalElement"/>
        <rdfs:range rdf:resource="http://www.w3.org/2001/XMLSchema#string"/>
        <rdfs:label>has chemical symbol</rdfs:label>
        <skos:definition>A data property linking an element with its chemical symbol.</skos:definition>
    </owl:DatatypeProperty>
    


    <!-- http://purls.helmholtz-metadaten.de/cmso/hasComponent_x -->

    <owl:DatatypeProperty rdf:about="http://purls.helmholtz-metadaten.de/cmso/hasComponent_x">
        <rdfs:domain rdf:resource="http://purls.helmholtz-metadaten.de/cmso/Vector"/>
        <rdfs:range rdf:resource="http://www.w3.org/2001/XMLSchema#float"/>
        <rdfs:label>has component x</rdfs:label>
        <skos:definition>A data property linking a vector with its component on the x axis.</skos:definition>
    </owl:DatatypeProperty>
    


    <!-- http://purls.helmholtz-metadaten.de/cmso/hasComponent_y -->

    <owl:DatatypeProperty rdf:about="http://purls.helmholtz-metadaten.de/cmso/hasComponent_y">
        <rdfs:domain rdf:resource="http://purls.helmholtz-metadaten.de/cmso/Vector"/>
        <rdfs:range rdf:resource="http://www.w3.org/2001/XMLSchema#float"/>
        <rdfs:label>has component y</rdfs:label>
        <skos:definition>A data property linking a vector with its component on the y axis.</skos:definition>
    </owl:DatatypeProperty>
    


    <!-- http://purls.helmholtz-metadaten.de/cmso/hasComponent_z -->

    <owl:DatatypeProperty rdf:about="http://purls.helmholtz-metadaten.de/cmso/hasComponent_z">
        <rdfs:domain rdf:resource="http://purls.helmholtz-metadaten.de/cmso/Vector"/>
        <rdfs:range rdf:resource="http://www.w3.org/2001/XMLSchema#float"/>
        <rdfs:label>has component z</rdfs:label>
        <skos:definition>A data property linking a vector with its component on the z axis.</skos:definition>
    </owl:DatatypeProperty>
    


    <!-- http://purls.helmholtz-metadaten.de/cmso/hasCoordinationNumber -->

    <owl:DatatypeProperty rdf:about="http://purls.helmholtz-metadaten.de/cmso/hasCoordinationNumber">
        <rdfs:domain rdf:resource="http://purls.helmholtz-metadaten.de/cmso/Atom"/>
        <rdfs:range rdf:resource="http://www.w3.org/2001/XMLSchema#integer"/>
        <rdfs:label>has coordination number</rdfs:label>
        <skos:definition>A data property linking an atom with its coordination number. The coordination number of an atom in an extended structure is the number of nearest neighbors.</skos:definition>
    </owl:DatatypeProperty>
    


    <!-- http://purls.helmholtz-metadaten.de/cmso/hasElementRatio -->

    <owl:DatatypeProperty rdf:about="http://purls.helmholtz-metadaten.de/cmso/hasElementRatio">
        <rdfs:domain rdf:resource="http://purls.helmholtz-metadaten.de/cmso/Material"/>
        <rdfs:range rdf:resource="http://www.w3.org/2001/XMLSchema#string"/>
        <rdfs:label>has element ratio</rdfs:label>
        <skos:definition>A data property linking a material with the ratio or fraction of an element that constitutes it. Comment: indicated with a value from 0 to 1.</skos:definition>
    </owl:DatatypeProperty>
    


    <!-- http://purls.helmholtz-metadaten.de/cmso/hasLength_x -->

    <owl:DatatypeProperty rdf:about="http://purls.helmholtz-metadaten.de/cmso/hasLength_x">
        <rdfs:domain>
            <owl:Class>
                <owl:unionOf rdf:parseType="Collection">
                    <rdf:Description rdf:about="http://purls.helmholtz-metadaten.de/cmso/LatticeParameter"/>
                    <rdf:Description rdf:about="http://purls.helmholtz-metadaten.de/cmso/Length"/>
                </owl:unionOf>
            </owl:Class>
        </rdfs:domain>
        <rdfs:range rdf:resource="http://www.w3.org/2001/XMLSchema#float"/>
        <rdfs:label>has length x</rdfs:label>
        <skos:definition>A data property linking a length to the measurement in the x axis.</skos:definition>
    </owl:DatatypeProperty>
    


    <!-- http://purls.helmholtz-metadaten.de/cmso/hasLength_y -->

    <owl:DatatypeProperty rdf:about="http://purls.helmholtz-metadaten.de/cmso/hasLength_y">
        <rdfs:domain>
            <owl:Class>
                <owl:unionOf rdf:parseType="Collection">
                    <rdf:Description rdf:about="http://purls.helmholtz-metadaten.de/cmso/LatticeParameter"/>
                    <rdf:Description rdf:about="http://purls.helmholtz-metadaten.de/cmso/Length"/>
                </owl:unionOf>
            </owl:Class>
        </rdfs:domain>
        <rdfs:range rdf:resource="http://www.w3.org/2001/XMLSchema#float"/>
        <rdfs:label>has length y</rdfs:label>
        <skos:definition>A data property linking a length to the measurement in the y axis.</skos:definition>
    </owl:DatatypeProperty>
    


    <!-- http://purls.helmholtz-metadaten.de/cmso/hasLength_z -->

    <owl:DatatypeProperty rdf:about="http://purls.helmholtz-metadaten.de/cmso/hasLength_z">
        <rdfs:domain>
            <owl:Class>
                <owl:unionOf rdf:parseType="Collection">
                    <rdf:Description rdf:about="http://purls.helmholtz-metadaten.de/cmso/LatticeParameter"/>
                    <rdf:Description rdf:about="http://purls.helmholtz-metadaten.de/cmso/Length"/>
                </owl:unionOf>
            </owl:Class>
        </rdfs:domain>
        <rdfs:range rdf:resource="http://www.w3.org/2001/XMLSchema#float"/>
        <rdfs:label>has length z</rdfs:label>
        <skos:definition>A data property linking a length to the measurement in the z axis.</skos:definition>
    </owl:DatatypeProperty>
    


    <!-- http://purls.helmholtz-metadaten.de/cmso/hasName -->

    <owl:DatatypeProperty rdf:about="http://purls.helmholtz-metadaten.de/cmso/hasName">
        <rdfs:domain rdf:resource="http://www.w3.org/2002/07/owl#Thing"/>
        <rdfs:range rdf:resource="http://www.w3.org/2001/XMLSchema#string"/>
        <rdfs:label>has name</rdfs:label>
        <skos:definition>A data property linking an entity with its name.</skos:definition>
    </owl:DatatypeProperty>
    


    <!-- http://purls.helmholtz-metadaten.de/cmso/hasNumberOfAtoms -->

    <owl:DatatypeProperty rdf:about="http://purls.helmholtz-metadaten.de/cmso/hasNumberOfAtoms">
        <rdfs:domain rdf:resource="http://purls.helmholtz-metadaten.de/cmso/AtomicScaleSample"/>
        <rdfs:range rdf:resource="http://www.w3.org/2001/XMLSchema#integer"/>
        <rdfs:label>has number of atoms</rdfs:label>
        <skos:definition>A data property linking an atomic scale sample with the number of atoms it contains.</skos:definition>
    </owl:DatatypeProperty>
    


    <!-- http://purls.helmholtz-metadaten.de/cmso/hasReference -->

    <owl:DatatypeProperty rdf:about="http://purls.helmholtz-metadaten.de/cmso/hasReference">
        <rdfs:domain rdf:resource="http://www.w3.org/2002/07/owl#Thing"/>
        <rdfs:range rdf:resource="http://www.w3.org/2000/01/rdf-schema#Literal"/>
        <rdfs:label>has reference</rdfs:label>
        <skos:definition>A data property linking an entity with a reference (e.g. bibliographic) to another resource.</skos:definition>
    </owl:DatatypeProperty>
    


    <!-- http://purls.helmholtz-metadaten.de/cmso/hasRepetition_x -->

    <owl:DatatypeProperty rdf:about="http://purls.helmholtz-metadaten.de/cmso/hasRepetition_x">
        <rdfs:domain rdf:resource="http://purls.helmholtz-metadaten.de/cmso/SimulationCell"/>
        <rdfs:range rdf:resource="http://www.w3.org/2001/XMLSchema#float"/>
        <rdfs:label>has repetition x</rdfs:label>
        <skos:definition>A data property linking a simulation cell with its number of repetitions in the x direction.</skos:definition>
    </owl:DatatypeProperty>
    


    <!-- http://purls.helmholtz-metadaten.de/cmso/hasRepetition_y -->

    <owl:DatatypeProperty rdf:about="http://purls.helmholtz-metadaten.de/cmso/hasRepetition_y">
        <rdfs:domain rdf:resource="http://purls.helmholtz-metadaten.de/cmso/SimulationCell"/>
        <rdfs:range rdf:resource="http://www.w3.org/2001/XMLSchema#float"/>
        <rdfs:label>has repetition y</rdfs:label>
        <skos:definition>A data property linking a simulation cell with its number of repetitions in the y direction.</skos:definition>
    </owl:DatatypeProperty>
    


    <!-- http://purls.helmholtz-metadaten.de/cmso/hasRepetition_z -->

    <owl:DatatypeProperty rdf:about="http://purls.helmholtz-metadaten.de/cmso/hasRepetition_z">
        <rdfs:domain rdf:resource="http://purls.helmholtz-metadaten.de/cmso/SimulationCell"/>
        <rdfs:range rdf:resource="http://www.w3.org/2001/XMLSchema#float"/>
        <rdfs:label>has repetition z</rdfs:label>
        <skos:definition>A data property linking a simulation cell with its number of repetitions in the z direction.</skos:definition>
    </owl:DatatypeProperty>
    


    <!-- http://purls.helmholtz-metadaten.de/cmso/hasSpaceGroupNumber -->

    <owl:DatatypeProperty rdf:about="http://purls.helmholtz-metadaten.de/cmso/hasSpaceGroupNumber">
        <rdfs:domain rdf:resource="http://purls.helmholtz-metadaten.de/cmso/SpaceGroup"/>
        <rdfs:range rdf:resource="http://www.w3.org/2001/XMLSchema#integer"/>
        <rdfs:label>has space group number</rdfs:label>
        <skos:definition>A data property linking a crystal structure with its space group number.</skos:definition>
    </owl:DatatypeProperty>
    


    <!-- http://purls.helmholtz-metadaten.de/cmso/hasSpaceGroupSymbol -->

    <owl:DatatypeProperty rdf:about="http://purls.helmholtz-metadaten.de/cmso/hasSpaceGroupSymbol">
        <rdfs:subPropertyOf rdf:resource="http://purls.helmholtz-metadaten.de/cmso/hasSymbol"/>
        <rdfs:domain rdf:resource="http://purls.helmholtz-metadaten.de/cmso/SpaceGroup"/>
        <rdfs:range rdf:resource="http://www.w3.org/2001/XMLSchema#string"/>
        <rdfs:label>has space group symbol</rdfs:label>
        <skos:definition>A data property linking a crystal structure with its space group symbol.</skos:definition>
    </owl:DatatypeProperty>
    


    <!-- http://purls.helmholtz-metadaten.de/cmso/hasSymbol -->

    <owl:DatatypeProperty rdf:about="http://purls.helmholtz-metadaten.de/cmso/hasSymbol">
        <rdfs:domain rdf:resource="http://www.w3.org/2002/07/owl#Thing"/>
        <rdfs:label>has symbol</rdfs:label>
        <skos:definition>A data property linking an entity with its symbol.</skos:definition>
    </owl:DatatypeProperty>
    


    <!-- http://purls.helmholtz-metadaten.de/cmso/hasValue -->

    <owl:DatatypeProperty rdf:about="http://purls.helmholtz-metadaten.de/cmso/hasValue">
        <rdfs:domain rdf:resource="http://purls.helmholtz-metadaten.de/cmso/CalculatedProperty"/>
        <rdfs:range rdf:resource="http://www.w3.org/2000/01/rdf-schema#Literal"/>
        <rdfs:label>has value</rdfs:label>
        <skos:definition>A data property linking a calculated property to its value.</skos:definition>
    </owl:DatatypeProperty>
    


    <!-- http://purls.helmholtz-metadaten.de/cmso/hasVolume -->

    <owl:DatatypeProperty rdf:about="http://purls.helmholtz-metadaten.de/cmso/hasVolume">
        <rdfs:domain rdf:resource="http://purls.helmholtz-metadaten.de/cmso/SimulationCell"/>
        <rdfs:range rdf:resource="http://www.w3.org/2001/XMLSchema#float"/>
        <rdfs:label>has volume</rdfs:label>
        <skos:definition>A data property linking a simulation cell with its volume. Comment: the unit of the volume is indicated by the unit of the simulation cell length.</skos:definition>
    </owl:DatatypeProperty>
    


    <!-- 
    ///////////////////////////////////////////////////////////////////////////////////////
    //
    // Classes
    //
    ///////////////////////////////////////////////////////////////////////////////////////
     -->

    


    <!-- http://purls.helmholtz-metadaten.de/cmso/AmorphousMaterial -->

    <owl:Class rdf:about="http://purls.helmholtz-metadaten.de/cmso/AmorphousMaterial">
        <rdfs:subClassOf rdf:resource="http://purls.helmholtz-metadaten.de/cmso/Material"/>
        <rdfs:label>Amorphous Material</rdfs:label>
        <skos:altLabel>Amorphous Solid</skos:altLabel>
        <skos:altLabel>Non-crystalline Solid</skos:altLabel>
        <skos:definition>An amorphous material or solid is a material which has no defined long-range periodicity.</skos:definition>
    </owl:Class>
    


    <!-- http://purls.helmholtz-metadaten.de/cmso/Angle -->

    <owl:Class rdf:about="http://purls.helmholtz-metadaten.de/cmso/Angle">
        <rdfs:label>Angle</rdfs:label>
        <skos:definition>An angle is a measure of the the space (usually in degrees) between two intersecting lines at the point where they meet or vertex.</skos:definition>
    </owl:Class>
    


    <!-- http://purls.helmholtz-metadaten.de/cmso/Atom -->

    <owl:Class rdf:about="http://purls.helmholtz-metadaten.de/cmso/Atom">
        <rdfs:subClassOf rdf:resource="http://purls.helmholtz-metadaten.de/cmso/ChemicalSpecies"/>
        <rdfs:comment>Reference: https://goldbook.iupac.org/terms/view/A00493</rdfs:comment>
        <rdfs:label>Atom</rdfs:label>
        <skos:definition>Smallest particle still characterizing a chemical element. It consists of a nucleus of a positive charge (Z is the proton number and e the elementary charge) carrying almost all its mass (more than 99.9%) and Z electrons determining its size.</skos:definition>
    </owl:Class>
    


    <!-- http://purls.helmholtz-metadaten.de/cmso/AtomicScaleSample -->

    <owl:Class rdf:about="http://purls.helmholtz-metadaten.de/cmso/AtomicScaleSample">
        <rdfs:subClassOf rdf:resource="http://purls.helmholtz-metadaten.de/cmso/ComputationalSample"/>
        <rdfs:label>Atomic Scale Sample</rdfs:label>
        <skos:definition>Atomic scale sample is a computational sample in the atomic length scale.</skos:definition>
    </owl:Class>
    


    <!-- http://purls.helmholtz-metadaten.de/cmso/Basis -->

    <owl:Class rdf:about="http://purls.helmholtz-metadaten.de/cmso/Basis">
        <rdfs:label>Basis</rdfs:label>
        <skos:definition>The basis of a crystal indicates the arrangement or position of atoms in the crystal lattice.</skos:definition>
    </owl:Class>
    


    <!-- http://purls.helmholtz-metadaten.de/cmso/CalculatedProperty -->

    <owl:Class rdf:about="http://purls.helmholtz-metadaten.de/cmso/CalculatedProperty">
        <rdfs:label>Calculated Property</rdfs:label>
        <skos:definition>A calculated property is a property of a material resulting from a calculation or simulation.</skos:definition>
    </owl:Class>
    


    <!-- http://purls.helmholtz-metadaten.de/cmso/ChemicalElement -->

    <owl:Class rdf:about="http://purls.helmholtz-metadaten.de/cmso/ChemicalElement">
        <rdfs:comment>Reference: https://goldbook.iupac.org/terms/view/C01022</rdfs:comment>
        <rdfs:label>Chemical Element</rdfs:label>
        <skos:definition>A species of atoms; all atoms with the same number of protons in the atomic nucleus.</skos:definition>
    </owl:Class>
    


    <!-- http://purls.helmholtz-metadaten.de/cmso/ChemicalSpecies -->

    <owl:Class rdf:about="http://purls.helmholtz-metadaten.de/cmso/ChemicalSpecies">
        <rdfs:comment>In this context, it refers to either an atom, ion or molecule.</rdfs:comment>
        <rdfs:comment>Reference: https://goldbook.iupac.org/terms/view/CT01038</rdfs:comment>
        <rdfs:label>Chemical Species</rdfs:label>
        <skos:definition>A chemical species is an ensemble of chemically identical atomic or molecular structural units in a solid array. Comment: In this context, it refers to either an atom, ion or molecule.</skos:definition>
    </owl:Class>
    


    <!-- http://purls.helmholtz-metadaten.de/cmso/ComputationalSample -->

    <owl:Class rdf:about="http://purls.helmholtz-metadaten.de/cmso/ComputationalSample">
        <rdfs:label>Computational Sample</rdfs:label>
        <skos:definition>A computational sample is a representative system of a material for analysis through computational methods in the context of materials science.</skos:definition>
    </owl:Class>
    


    <!-- http://purls.helmholtz-metadaten.de/cmso/CrystalDefect -->

    <owl:Class rdf:about="http://purls.helmholtz-metadaten.de/cmso/CrystalDefect">
        <rdfs:label>Crystal Defect</rdfs:label>
        <skos:altLabel>Crystallographic Defect</skos:altLabel>
        <skos:definition>A crystal defect is an imperfection or irregularity in the atomic arrangement of a crystalline solid.</skos:definition>
    </owl:Class>
    


    <!-- http://purls.helmholtz-metadaten.de/cmso/CrystalStructure -->

    <owl:Class rdf:about="http://purls.helmholtz-metadaten.de/cmso/CrystalStructure">
        <rdfs:subClassOf rdf:resource="http://purls.helmholtz-metadaten.de/cmso/Structure"/>
        <rdfs:comment>In this context, the crystal structure refers to the idealized state, while the defect information is represented elsewhere (see Crystal Defect).</rdfs:comment>
        <rdfs:label>Crystal Structure</rdfs:label>
        <skos:definition>Crystal structure is the arrangement of atoms or molecules in the solid state. Crystal structure also involves consideration of defects, or abnormalities, in the idealized atomic/molecular arrangements.</skos:definition>
    </owl:Class>
    


    <!-- http://purls.helmholtz-metadaten.de/cmso/CrystallineMaterial -->

    <owl:Class rdf:about="http://purls.helmholtz-metadaten.de/cmso/CrystallineMaterial">
        <rdfs:subClassOf rdf:resource="http://purls.helmholtz-metadaten.de/cmso/Material"/>
        <rdfs:label>Crystalline Material</rdfs:label>
        <skos:altLabel>Crystal</skos:altLabel>
        <skos:altLabel>Crystalline Solid</skos:altLabel>
        <skos:definition>A crystalline material or solid is a material in which atoms or molecules are arranged in a highly ordered and repeating pattern, forming a three-dimensional crystal lattice.</skos:definition>
    </owl:Class>
    


    <!-- http://purls.helmholtz-metadaten.de/cmso/LatticeAngle -->

    <owl:Class rdf:about="http://purls.helmholtz-metadaten.de/cmso/LatticeAngle">
        <rdfs:subClassOf rdf:resource="http://purls.helmholtz-metadaten.de/cmso/Angle"/>
        <rdfs:label>Lattice Angle</rdfs:label>
        <skos:definition>The lattice angle refers to the angles between the crystallographic axes.</skos:definition>
    </owl:Class>
    


    <!-- http://purls.helmholtz-metadaten.de/cmso/LatticeParameter -->

    <owl:Class rdf:about="http://purls.helmholtz-metadaten.de/cmso/LatticeParameter">
        <rdfs:subClassOf>
            <owl:Class>
                <owl:unionOf rdf:parseType="Collection">
                    <rdf:Description rdf:about="http://purls.helmholtz-metadaten.de/cmso/Length"/>
                    <rdf:Description rdf:about="http://purls.helmholtz-metadaten.de/cmso/UnitCell"/>
                </owl:unionOf>
            </owl:Class>
        </rdfs:subClassOf>
        <rdfs:comment>The lattice angles can also be considered lattice parameters (see Lattice Angles)</rdfs:comment>
        <rdfs:label>Lattice Parameter</rdfs:label>
        <skos:altLabel>Lattice Constant</skos:altLabel>
        <skos:definition>The lattice parameter is the measurement of length of the unit cell of the crystal lattice.</skos:definition>
    </owl:Class>
    


    <!-- http://purls.helmholtz-metadaten.de/cmso/LatticeVector -->

    <owl:Class rdf:about="http://purls.helmholtz-metadaten.de/cmso/LatticeVector">
        <rdfs:subClassOf rdf:resource="http://purls.helmholtz-metadaten.de/cmso/Vector"/>
        <rdfs:comment>Note that it differs from the simulation cell vector.</rdfs:comment>
        <rdfs:label>Lattice Vector</rdfs:label>
        <skos:definition>A lattice vector is a vector that defines the lattice of the crystal structure.</skos:definition>
    </owl:Class>
    


    <!-- http://purls.helmholtz-metadaten.de/cmso/Length -->

    <owl:Class rdf:about="http://purls.helmholtz-metadaten.de/cmso/Length">
        <rdfs:label>Length</rdfs:label>
        <skos:definition>Length is a measure of distance.</skos:definition>
    </owl:Class>
    


    <!-- http://purls.helmholtz-metadaten.de/cmso/MacroscaleSample -->

    <owl:Class rdf:about="http://purls.helmholtz-metadaten.de/cmso/MacroscaleSample">
        <rdfs:subClassOf rdf:resource="http://purls.helmholtz-metadaten.de/cmso/ComputationalSample"/>
        <rdfs:label>Macroscale Sample</rdfs:label>
        <skos:altLabel>Macro Scale Sample</skos:altLabel>
        <skos:definition>Macroscale sample is a computational sample in the macroscale.</skos:definition>
    </owl:Class>
    


    <!-- http://purls.helmholtz-metadaten.de/cmso/Material -->

    <owl:Class rdf:about="http://purls.helmholtz-metadaten.de/cmso/Material">
        <rdfs:comment>Reference: https://web.archive.org/web/20100801234616/http://www.nature.com/nmat/authors/index.html</rdfs:comment>
        <rdfs:label>Material</rdfs:label>
        <skos:definition>Materials are substances in the condensed states (liquid, solid, colloidal) designed or manipulated for technological ends.</skos:definition>
    </owl:Class>
    


    <!-- http://purls.helmholtz-metadaten.de/cmso/MesoscaleSample -->

    <owl:Class rdf:about="http://purls.helmholtz-metadaten.de/cmso/MesoscaleSample">
        <rdfs:subClassOf rdf:resource="http://purls.helmholtz-metadaten.de/cmso/ComputationalSample"/>
        <rdfs:label>Mesoscale Sample</rdfs:label>
        <skos:altLabel>Meso Scale Sample</skos:altLabel>
        <skos:definition>Mesoscale sample is a computational sample in the mesoscale.</skos:definition>
    </owl:Class>
    


    <!-- http://purls.helmholtz-metadaten.de/cmso/MicroscaleSample -->

    <owl:Class rdf:about="http://purls.helmholtz-metadaten.de/cmso/MicroscaleSample">
        <rdfs:subClassOf rdf:resource="http://purls.helmholtz-metadaten.de/cmso/ComputationalSample"/>
        <rdfs:label>Microscale Sample</rdfs:label>
        <skos:altLabel>Micro Scale Sample</skos:altLabel>
        <skos:definition>Microscale sample is a computational sample in the microscale.</skos:definition>
    </owl:Class>
    


    <!-- http://purls.helmholtz-metadaten.de/cmso/Microstructure -->

    <owl:Class rdf:about="http://purls.helmholtz-metadaten.de/cmso/Microstructure">
        <rdfs:subClassOf rdf:resource="http://purls.helmholtz-metadaten.de/cmso/Structure"/>
        <rdfs:label>Microstructure</rdfs:label>
        <skos:definition>The microstructure is the structure or arrangement of all components (atomic arrangement, defects, phases, etc.) of the material at the microscale.</skos:definition>
    </owl:Class>
    


    <!-- http://purls.helmholtz-metadaten.de/cmso/Molecule -->

    <owl:Class rdf:about="http://purls.helmholtz-metadaten.de/cmso/Molecule">
        <rdfs:subClassOf rdf:resource="http://purls.helmholtz-metadaten.de/cmso/ChemicalSpecies"/>
        <rdfs:comment>Reference: https://goldbook.iupac.org/terms/view/M04002</rdfs:comment>
        <rdfs:label>Molecule</rdfs:label>
        <skos:definition>An electrically neutral entity consisting of more than one atom (n&gt;1). Rigorously, a molecule, in which n&gt;1 must correspond to a depression on the potential energy surface that is deep enough to confine at least one vibrational state.</skos:definition>
    </owl:Class>
    


    <!-- http://purls.helmholtz-metadaten.de/cmso/NanoscaleSample -->

    <owl:Class rdf:about="http://purls.helmholtz-metadaten.de/cmso/NanoscaleSample">
        <rdfs:subClassOf rdf:resource="http://purls.helmholtz-metadaten.de/cmso/ComputationalSample"/>
        <rdfs:label>Nanoscale Sample</rdfs:label>
        <skos:definition>Nanoscale sample is a computational sample in the nanoscale.</skos:definition>
    </owl:Class>
    


    <!-- http://purls.helmholtz-metadaten.de/cmso/PositionVector -->

    <owl:Class rdf:about="http://purls.helmholtz-metadaten.de/cmso/PositionVector">
        <rdfs:subClassOf rdf:resource="http://purls.helmholtz-metadaten.de/cmso/Vector"/>
        <rdfs:comment>Cartesian coordinates are preferred over direct (or fractional) coordinates.</rdfs:comment>
        <rdfs:label>Position Vector</rdfs:label>
        <skos:definition>The position vector is a vector that represents the position of the atoms.</skos:definition>
    </owl:Class>
    


    <!-- http://purls.helmholtz-metadaten.de/cmso/SimulationCell -->

    <owl:Class rdf:about="http://purls.helmholtz-metadaten.de/cmso/SimulationCell">
        <rdfs:label>Simulation Cell</rdfs:label>
        <skos:altLabel>Box</skos:altLabel>
        <skos:altLabel>Supercell</skos:altLabel>
        <skos:definition>A simulation cell is a representation of the structure or system to be simulated. It is often a three-dimensional box (although not necessarily), where information about the crystal structure and material is contained.</skos:definition>
    </owl:Class>
    


    <!-- http://purls.helmholtz-metadaten.de/cmso/SimulationCellAngle -->

    <owl:Class rdf:about="http://purls.helmholtz-metadaten.de/cmso/SimulationCellAngle">
        <rdfs:subClassOf rdf:resource="http://purls.helmholtz-metadaten.de/cmso/Angle"/>
        <rdfs:label>Simulation Cell Angle</rdfs:label>
        <skos:definition>The simulation cell angle refers to the angles of the simulation cell in each direction.</skos:definition>
    </owl:Class>
    


    <!-- http://purls.helmholtz-metadaten.de/cmso/SimulationCellLength -->

    <owl:Class rdf:about="http://purls.helmholtz-metadaten.de/cmso/SimulationCellLength">
        <rdfs:subClassOf rdf:resource="http://purls.helmholtz-metadaten.de/cmso/Length"/>
        <rdfs:label>Simulation Cell Length</rdfs:label>
        <skos:altLabel>Box length</skos:altLabel>
        <skos:definition>The simulation cell length refers to the length (dimension) of the simulation cell or box.</skos:definition>
    </owl:Class>
    


    <!-- http://purls.helmholtz-metadaten.de/cmso/SimulationCellVector -->

    <owl:Class rdf:about="http://purls.helmholtz-metadaten.de/cmso/SimulationCellVector">
        <rdfs:subClassOf rdf:resource="http://purls.helmholtz-metadaten.de/cmso/Vector"/>
        <rdfs:comment>Note that it differs from the lattice vector.</rdfs:comment>
        <rdfs:label>Simulation Cell Vector</rdfs:label>
        <skos:definition>The simulation cell vector is a vector that defines the simulation cell or box.</skos:definition>
    </owl:Class>
    


    <!-- http://purls.helmholtz-metadaten.de/cmso/SpaceGroup -->

    <owl:Class rdf:about="http://purls.helmholtz-metadaten.de/cmso/SpaceGroup">
        <rdfs:label>Space Group</rdfs:label>
        <skos:definition>The space group represents the symmetry properties of the crystal. In three-dimensions, space groups are classified in 230 distinct groups.</skos:definition>
    </owl:Class>
    


    <!-- http://purls.helmholtz-metadaten.de/cmso/Structure -->

    <owl:Class rdf:about="http://purls.helmholtz-metadaten.de/cmso/Structure">
        <rdfs:comment>Reference: https://www.merriam-webster.com/dictionary/structure</rdfs:comment>
        <rdfs:label>Structure</rdfs:label>
        <skos:definition>Structure is the the arrangement of particles or parts in a substance or body.</skos:definition>
    </owl:Class>
    


    <!-- http://purls.helmholtz-metadaten.de/cmso/UnitCell -->

    <owl:Class rdf:about="http://purls.helmholtz-metadaten.de/cmso/UnitCell">
        <rdfs:label>Unit Cell</rdfs:label>
        <skos:definition>The unit cell is the smallest repeating unit of the crystal structure which contains the overal symmetry of the crystal. The entire crystal lattice can be generated by repeating the unit cell in three dimensions.</skos:definition>
    </owl:Class>
    


    <!-- http://purls.helmholtz-metadaten.de/cmso/Vector -->

    <owl:Class rdf:about="http://purls.helmholtz-metadaten.de/cmso/Vector">
        <rdfs:label>Vector</rdfs:label>
        <skos:definition>Vector is a quantity that has a magnitude and direction.</skos:definition>
    </owl:Class>
    


    <!-- http://qudt.org/schema/qudt/Unit -->

    <owl:Class rdf:about="http://qudt.org/schema/qudt/Unit">
        <terms:description rdf:datatype="http://qudt.org/schema/qudt/LatexString">A unit of measure, or unit, is a particular quantity value that has been chosen as a scale for measuring other quantities the same kind (more generally of equivalent dimension). For example, the meter is a quantity of length that has been rigorously defined and standardized by the BIPM (International Board of Weights and Measures). Any measurement of the length can be expressed as a number multiplied by the unit meter. More formally, the value of a physical quantity Q with respect to a unit (U) is expressed as the scalar multiple of a real number (n) and U, as  \(Q = nU\).</terms:description>
        <rdfs:isDefinedBy rdf:resource="http://qudt.org/2.1/schema/qudt"/>
        <rdfs:label>Unit</rdfs:label>
    </owl:Class>
    


    <!-- 
    ///////////////////////////////////////////////////////////////////////////////////////
    //
    // Annotations
    //
    ///////////////////////////////////////////////////////////////////////////////////////
     -->

    <rdf:Description rdf:about="http://www.w3.org/2004/02/skos/core#Collection">
        <skos:definition xml:lang="en">A meaningful collection of concepts.</skos:definition>
    </rdf:Description>
    <rdf:Description rdf:about="http://www.w3.org/2004/02/skos/core#Concept">
        <skos:definition xml:lang="en">An idea or notion; a unit of thought.</skos:definition>
    </rdf:Description>
    <rdf:Description rdf:about="http://www.w3.org/2004/02/skos/core#ConceptScheme">
        <skos:definition xml:lang="en">A set of concepts, optionally including statements about semantic relationships between those concepts.</skos:definition>
        <skos:example xml:lang="en">Thesauri, classification schemes, subject heading lists, taxonomies, &apos;folksonomies&apos;, and other types of controlled vocabulary are all examples of concept schemes. Concept schemes are also embedded in glossaries and terminologies.</skos:example>
    </rdf:Description>
    <rdf:Description rdf:about="http://www.w3.org/2004/02/skos/core#OrderedCollection">
        <skos:definition xml:lang="en">An ordered collection of concepts, where both the grouping and the ordering are meaningful.</skos:definition>
    </rdf:Description>
    <rdf:Description rdf:about="http://www.w3.org/2004/02/skos/core#broadMatch">
        <skos:definition xml:lang="en">skos:broadMatch is used to state a hierarchical mapping link between two conceptual resources in different concept schemes.</skos:definition>
    </rdf:Description>
    <rdf:Description rdf:about="http://www.w3.org/2004/02/skos/core#broader">
        <skos:definition xml:lang="en">Relates a concept to a concept that is more general in meaning.</skos:definition>
    </rdf:Description>
    <rdf:Description rdf:about="http://www.w3.org/2004/02/skos/core#broaderTransitive">
        <skos:definition>skos:broaderTransitive is a transitive superproperty of skos:broader.</skos:definition>
    </rdf:Description>
    <rdf:Description rdf:about="http://www.w3.org/2004/02/skos/core#changeNote">
        <skos:definition xml:lang="en">A note about a modification to a concept.</skos:definition>
    </rdf:Description>
    <rdf:Description rdf:about="http://www.w3.org/2004/02/skos/core#closeMatch">
        <skos:definition xml:lang="en">skos:closeMatch is used to link two concepts that are sufficiently similar that they can be used interchangeably in some information retrieval applications. In order to avoid the possibility of &quot;compound errors&quot; when combining mappings across more than two concept schemes, skos:closeMatch is not declared to be a transitive property.</skos:definition>
    </rdf:Description>
    <rdf:Description rdf:about="http://www.w3.org/2004/02/skos/core#editorialNote">
        <skos:definition xml:lang="en">A note for an editor, translator or maintainer of the vocabulary.</skos:definition>
    </rdf:Description>
    <rdf:Description rdf:about="http://www.w3.org/2004/02/skos/core#exactMatch">
        <skos:definition xml:lang="en">skos:exactMatch is used to link two concepts, indicating a high degree of confidence that the concepts can be used interchangeably across a wide range of information retrieval applications. skos:exactMatch is a transitive property, and is a sub-property of skos:closeMatch.</skos:definition>
    </rdf:Description>
    <rdf:Description rdf:about="http://www.w3.org/2004/02/skos/core#hasTopConcept">
        <skos:definition xml:lang="en">Relates, by convention, a concept scheme to a concept which is topmost in the broader/narrower concept hierarchies for that scheme, providing an entry point to these hierarchies.</skos:definition>
    </rdf:Description>
    <rdf:Description rdf:about="http://www.w3.org/2004/02/skos/core#hiddenLabel">
        <skos:definition xml:lang="en">A lexical label for a resource that should be hidden when generating visual displays of the resource, but should still be accessible to free text search operations.</skos:definition>
    </rdf:Description>
    <rdf:Description rdf:about="http://www.w3.org/2004/02/skos/core#historyNote">
        <skos:definition xml:lang="en">A note about the past state/use/meaning of a concept.</skos:definition>
    </rdf:Description>
    <rdf:Description rdf:about="http://www.w3.org/2004/02/skos/core#inScheme">
        <skos:definition xml:lang="en">Relates a resource (for example a concept) to a concept scheme in which it is included.</skos:definition>
    </rdf:Description>
    <rdf:Description rdf:about="http://www.w3.org/2004/02/skos/core#mappingRelation">
        <skos:definition xml:lang="en">Relates two concepts coming, by convention, from different schemes, and that have comparable meanings</skos:definition>
    </rdf:Description>
    <rdf:Description rdf:about="http://www.w3.org/2004/02/skos/core#member">
        <skos:definition xml:lang="en">Relates a collection to one of its members.</skos:definition>
    </rdf:Description>
    <rdf:Description rdf:about="http://www.w3.org/2004/02/skos/core#memberList">
        <skos:definition xml:lang="en">Relates an ordered collection to the RDF list containing its members.</skos:definition>
    </rdf:Description>
    <rdf:Description rdf:about="http://www.w3.org/2004/02/skos/core#narrowMatch">
        <skos:definition xml:lang="en">skos:narrowMatch is used to state a hierarchical mapping link between two conceptual resources in different concept schemes.</skos:definition>
    </rdf:Description>
    <rdf:Description rdf:about="http://www.w3.org/2004/02/skos/core#narrower">
        <skos:definition xml:lang="en">Relates a concept to a concept that is more specific in meaning.</skos:definition>
    </rdf:Description>
    <rdf:Description rdf:about="http://www.w3.org/2004/02/skos/core#narrowerTransitive">
        <skos:definition>skos:narrowerTransitive is a transitive superproperty of skos:narrower.</skos:definition>
    </rdf:Description>
    <rdf:Description rdf:about="http://www.w3.org/2004/02/skos/core#notation">
        <skos:definition xml:lang="en">A notation, also known as classification code, is a string of characters such as &quot;T58.5&quot; or &quot;303.4833&quot; used to uniquely identify a concept within the scope of a given concept scheme.</skos:definition>
    </rdf:Description>
    <rdf:Description rdf:about="http://www.w3.org/2004/02/skos/core#related">
        <skos:definition xml:lang="en">Relates a concept to a concept with which there is an associative semantic relationship.</skos:definition>
    </rdf:Description>
    <rdf:Description rdf:about="http://www.w3.org/2004/02/skos/core#relatedMatch">
        <skos:definition xml:lang="en">skos:relatedMatch is used to state an associative mapping link between two conceptual resources in different concept schemes.</skos:definition>
    </rdf:Description>
    <rdf:Description rdf:about="http://www.w3.org/2004/02/skos/core#scopeNote">
        <skos:definition xml:lang="en">A note that helps to clarify the meaning and/or the use of a concept.</skos:definition>
    </rdf:Description>
    <rdf:Description rdf:about="http://www.w3.org/2004/02/skos/core#semanticRelation">
        <skos:definition xml:lang="en">Links a concept to a concept related by meaning.</skos:definition>
    </rdf:Description>
    <rdf:Description rdf:about="http://www.w3.org/2004/02/skos/core#topConceptOf">
        <skos:definition xml:lang="en">Relates a concept to the concept scheme that it is a top level concept of.</skos:definition>
    </rdf:Description>
</rdf:RDF>



<!-- Generated by the OWL API (version 4.5.9.2019-02-01T07:24:44Z) https://github.com/owlcs/owlapi -->

