<?xml version="1.0"?>
<rdf:RDF xmlns="http://www.semanticweb.org/a.azocar.guzman/ontologies/2023/5/untitled-ontology-21#"
     xml:base="http://www.semanticweb.org/a.azocar.guzman/ontologies/2023/5/untitled-ontology-21"
     xmlns:dc="http://purl.org/dc/elements/1.1/"
     xmlns:owl="http://www.w3.org/2002/07/owl#"
     xmlns:rdf="http://www.w3.org/1999/02/22-rdf-syntax-ns#"
     xmlns:xml="http://www.w3.org/XML/1998/namespace"
     xmlns:xsd="http://www.w3.org/2001/XMLSchema#"
     xmlns:rdfs="http://www.w3.org/2000/01/rdf-schema#"
     xmlns:skos="http://www.w3.org/2004/02/skos/core#"
     xmlns:terms="http://purl.org/dc/terms/">
    <owl:Ontology rdf:about="http://purls.helmholtz-metadaten.de/podo/">
        <terms:contributor>https://orcid.org/0000-0001-9560-4728</terms:contributor>
        <terms:contributor>https://orcid.org/0000-0002-5149-603X</terms:contributor>
        <terms:contributor>https://orcid.org/0000-0002-6776-1213</terms:contributor>
        <terms:contributor>https://orcid.org/0000-0003-0698-4891</terms:contributor>
        <terms:creator>https://orcid.org/0000-0001-7564-7990</terms:creator>
        <terms:description>PODO focuses on the description of point defects in crystalline materials.</terms:description>
        <terms:title>Point Defects Ontology (PODO)</terms:title>
    </owl:Ontology>
    


    <!-- 
    ///////////////////////////////////////////////////////////////////////////////////////
    //
    // Annotation properties
    //
    ///////////////////////////////////////////////////////////////////////////////////////
     -->

    


    <!-- http://purl.org/dc/elements/1.1/contributor -->

    <owl:AnnotationProperty rdf:about="http://purl.org/dc/elements/1.1/contributor"/>
    


    <!-- http://purl.org/dc/elements/1.1/creator -->

    <owl:AnnotationProperty rdf:about="http://purl.org/dc/elements/1.1/creator"/>
    


    <!-- http://purl.org/dc/elements/1.1/description -->

    <owl:AnnotationProperty rdf:about="http://purl.org/dc/elements/1.1/description"/>
    


    <!-- http://purl.org/dc/elements/1.1/title -->

    <owl:AnnotationProperty rdf:about="http://purl.org/dc/elements/1.1/title"/>
    


    <!-- http://purl.org/dc/terms/abstract -->

    <owl:AnnotationProperty rdf:about="http://purl.org/dc/terms/abstract">
        <rdfs:subPropertyOf rdf:resource="http://purl.org/dc/terms/description"/>
    </owl:AnnotationProperty>
    


    <!-- http://purl.org/dc/terms/alternative -->

    <owl:AnnotationProperty rdf:about="http://purl.org/dc/terms/alternative">
        <rdfs:subPropertyOf rdf:resource="http://purl.org/dc/terms/title"/>
    </owl:AnnotationProperty>
    


    <!-- http://purl.org/dc/terms/contributor -->

    <owl:AnnotationProperty rdf:about="http://purl.org/dc/terms/contributor">
        <rdfs:comment xml:lang="en-us">Examples of a Contributor include a person, an organization, or a service. Typically, the name of a Contributor should be used to indicate the entity.</rdfs:comment>
        <rdfs:label xml:lang="en-us">Contributor</rdfs:label>
        <skos:definition xml:lang="en-us">An entity responsible for making contributions to the resource.</skos:definition>
        <rdfs:subPropertyOf rdf:resource="http://purl.org/dc/elements/1.1/contributor"/>
        <rdfs:range rdf:resource="http://purl.org/dc/terms/Agent"/>
    </owl:AnnotationProperty>
    


    <!-- http://purl.org/dc/terms/creator -->

    <owl:AnnotationProperty rdf:about="http://purl.org/dc/terms/creator">
        <rdfs:comment xml:lang="en-us">Examples of a Creator include a person, an organization, or a service. Typically, the name of a Creator should be used to indicate the entity.</rdfs:comment>
        <rdfs:label xml:lang="en-us">Creator</rdfs:label>
        <skos:definition xml:lang="en-us">An entity primarily responsible for making the resource.</skos:definition>
        <rdfs:subPropertyOf rdf:resource="http://purl.org/dc/elements/1.1/creator"/>
        <rdfs:subPropertyOf rdf:resource="http://purl.org/dc/terms/contributor"/>
        <rdfs:range rdf:resource="http://purl.org/dc/terms/Agent"/>
    </owl:AnnotationProperty>
    


    <!-- http://purl.org/dc/terms/description -->

    <owl:AnnotationProperty rdf:about="http://purl.org/dc/terms/description">
        <rdfs:comment xml:lang="en-us">Description may include but is not limited to: an abstract, a table of contents, a graphical representation, or a free-text account of the resource.</rdfs:comment>
        <rdfs:label xml:lang="en-us">Description</rdfs:label>
        <skos:definition xml:lang="en-us">An account of the resource.</skos:definition>
        <rdfs:subPropertyOf rdf:resource="http://purl.org/dc/elements/1.1/description"/>
    </owl:AnnotationProperty>
    


    <!-- http://purl.org/dc/terms/tableOfContents -->

    <owl:AnnotationProperty rdf:about="http://purl.org/dc/terms/tableOfContents">
        <rdfs:subPropertyOf rdf:resource="http://purl.org/dc/terms/description"/>
    </owl:AnnotationProperty>
    


    <!-- http://purl.org/dc/terms/title -->

    <owl:AnnotationProperty rdf:about="http://purl.org/dc/terms/title">
        <rdfs:label xml:lang="en-us">Title</rdfs:label>
        <skos:definition xml:lang="en-us">A name given to the resource.</skos:definition>
        <skos:note xml:lang="en-us">In current practice, this term is used primarily with literal values; however, there are important uses with non-literal values as well. As of December 2007, the DCMI Usage Board is leaving this range unspecified pending an investigation of options.</skos:note>
        <rdfs:subPropertyOf rdf:resource="http://purl.org/dc/elements/1.1/title"/>
    </owl:AnnotationProperty>
    


    <!-- http://www.w3.org/2004/02/skos/core#altLabel -->

    <owl:AnnotationProperty rdf:about="http://www.w3.org/2004/02/skos/core#altLabel">
        <rdfs:comment xml:lang="en">The range of skos:altLabel is the class of RDF plain literals.</rdfs:comment>
        <rdfs:comment xml:lang="en">skos:prefLabel, skos:altLabel and skos:hiddenLabel are pairwise disjoint properties.</rdfs:comment>
        <rdfs:isDefinedBy rdf:resource="http://www.w3.org/2004/02/skos/core"/>
        <rdfs:label xml:lang="en">alternative label</rdfs:label>
        <skos:definition xml:lang="en">An alternative lexical label for a resource.</skos:definition>
        <skos:example xml:lang="en">Acronyms, abbreviations, spelling variants, and irregular plural/singular forms may be included among the alternative labels for a concept. Mis-spelled terms are normally included as hidden labels (see skos:hiddenLabel).</skos:example>
        <rdfs:subPropertyOf rdf:resource="http://www.w3.org/2000/01/rdf-schema#label"/>
    </owl:AnnotationProperty>
    


    <!-- http://www.w3.org/2004/02/skos/core#definition -->

    <owl:AnnotationProperty rdf:about="http://www.w3.org/2004/02/skos/core#definition">
        <rdfs:isDefinedBy rdf:resource="http://www.w3.org/2004/02/skos/core"/>
        <rdfs:label xml:lang="en">definition</rdfs:label>
        <skos:definition xml:lang="en">A statement or formal explanation of the meaning of a concept.</skos:definition>
        <rdfs:subPropertyOf rdf:resource="http://www.w3.org/2004/02/skos/core#note"/>
    </owl:AnnotationProperty>
    


    <!-- http://www.w3.org/2004/02/skos/core#example -->

    <owl:AnnotationProperty rdf:about="http://www.w3.org/2004/02/skos/core#example">
        <rdfs:isDefinedBy rdf:resource="http://www.w3.org/2004/02/skos/core"/>
        <rdfs:label xml:lang="en">example</rdfs:label>
        <skos:definition xml:lang="en">An example of the use of a concept.</skos:definition>
        <rdfs:subPropertyOf rdf:resource="http://www.w3.org/2004/02/skos/core#note"/>
    </owl:AnnotationProperty>
    


    <!-- http://www.w3.org/2004/02/skos/core#note -->

    <owl:AnnotationProperty rdf:about="http://www.w3.org/2004/02/skos/core#note">
        <skos:definition xml:lang="en">A general note, for any purpose.</skos:definition>
    </owl:AnnotationProperty>
    


    <!-- http://www.w3.org/2004/02/skos/core#prefLabel -->

    <owl:AnnotationProperty rdf:about="http://www.w3.org/2004/02/skos/core#prefLabel">
        <rdfs:comment xml:lang="en">A resource has no more than one value of skos:prefLabel per language tag, and no more than one value of skos:prefLabel without language tag.</rdfs:comment>
        <rdfs:comment xml:lang="en">The range of skos:prefLabel is the class of RDF plain literals.</rdfs:comment>
        <rdfs:comment xml:lang="en">skos:prefLabel, skos:altLabel and skos:hiddenLabel are pairwise
      disjoint properties.</rdfs:comment>
        <rdfs:isDefinedBy rdf:resource="http://www.w3.org/2004/02/skos/core"/>
        <rdfs:label xml:lang="en">preferred label</rdfs:label>
        <skos:definition xml:lang="en">The preferred lexical label for a resource, in a given language.</skos:definition>
        <rdfs:subPropertyOf rdf:resource="http://www.w3.org/2000/01/rdf-schema#label"/>
    </owl:AnnotationProperty>
    


    <!-- 
    ///////////////////////////////////////////////////////////////////////////////////////
    //
    // Data properties
    //
    ///////////////////////////////////////////////////////////////////////////////////////
     -->

    


    <!-- http://purls.helmholtz-metadaten.de/podo/hasNumberOfVacancies -->

    <owl:DatatypeProperty rdf:about="http://purls.helmholtz-metadaten.de/podo/hasNumberOfVacancies">
        <rdfs:label>has number of vacancies</rdfs:label>
        <skos:definition>A data property indicating the total number of vacancies in the crystal structure.</skos:definition>
    </owl:DatatypeProperty>
    


    <!-- http://purls.helmholtz-metadaten.de/podo/hasVacancyConcentration -->

    <owl:DatatypeProperty rdf:about="http://purls.helmholtz-metadaten.de/podo/hasVacancyConcentration">
        <rdfs:comment>Note that the vacancy concentration is given as a fraction, with a value from 0 to 1.</rdfs:comment>
        <rdfs:label>has vacancy concentration</rdfs:label>
        <skos:definition>A data property indicating the vacancy concentration.</skos:definition>
    </owl:DatatypeProperty>
    


    <!-- 
    ///////////////////////////////////////////////////////////////////////////////////////
    //
    // Classes
    //
    ///////////////////////////////////////////////////////////////////////////////////////
     -->

    


    <!-- http://purls.helmholtz-metadaten.de/podo/AntisiteDefect -->

    <owl:Class rdf:about="http://purls.helmholtz-metadaten.de/podo/AntisiteDefect">
        <rdfs:subClassOf rdf:resource="http://purls.helmholtz-metadaten.de/podo/PointDefect"/>
        <rdfs:comment>Reference: ISBN 978-1-119-45416-8</rdfs:comment>
        <rdfs:label>Antisite Defect</rdfs:label>
        <skos:definition>Antisite Defect is a point defect which occurs in ordered alloys or compounds when two atoms of different type switch positions.</skos:definition>
    </owl:Class>
    


    <!-- http://purls.helmholtz-metadaten.de/podo/FrenkelDefect -->

    <owl:Class rdf:about="http://purls.helmholtz-metadaten.de/podo/FrenkelDefect">
        <rdfs:subClassOf rdf:resource="http://purls.helmholtz-metadaten.de/podo/PointDefect"/>
        <rdfs:comment>Reference: ISBN 978-1-119-45416-8</rdfs:comment>
        <rdfs:label>Frenkel Defect</rdfs:label>
        <skos:altLabel>Frenkel Pair</skos:altLabel>
        <skos:definition>A Frenkel defect is a point defect which occurs in ionic crystals when an ion is removed to an interstitial position, leaving a vacancy behind.</skos:definition>
    </owl:Class>
    


    <!-- http://purls.helmholtz-metadaten.de/podo/Impurity -->

    <owl:Class rdf:about="http://purls.helmholtz-metadaten.de/podo/Impurity">
        <rdfs:subClassOf rdf:resource="http://purls.helmholtz-metadaten.de/podo/PointDefect"/>
        <rdfs:label>Impurity</rdfs:label>
        <skos:definition>An impurity is a point defect where foreign atoms (of different type as the host atom) enter the crystal lattice.</skos:definition>
    </owl:Class>
    


    <!-- http://purls.helmholtz-metadaten.de/podo/Interstitial -->

    <owl:Class rdf:about="http://purls.helmholtz-metadaten.de/podo/Interstitial">
        <rdfs:subClassOf rdf:resource="http://purls.helmholtz-metadaten.de/podo/PointDefect"/>
        <rdfs:label>Interstitial</rdfs:label>
        <skos:definition>An interstitial is a point defect where an atom occupies an interstitial site. In crystallography, interstitial sites are the empty space between the atoms (assuming a hard-sphere model).</skos:definition>
    </owl:Class>
    


    <!-- http://purls.helmholtz-metadaten.de/podo/InterstitialImpurity -->

    <owl:Class rdf:about="http://purls.helmholtz-metadaten.de/podo/InterstitialImpurity">
        <rdfs:subClassOf rdf:resource="http://purls.helmholtz-metadaten.de/podo/Impurity"/>
        <rdfs:subClassOf rdf:resource="http://purls.helmholtz-metadaten.de/podo/Interstitial"/>
        <rdfs:label>Interstitial Impurity</rdfs:label>
        <skos:definition>A interstitial impurity is a point defect where the atom occupying the interstitial site is of a different type as the matrix.</skos:definition>
    </owl:Class>
    


    <!-- http://purls.helmholtz-metadaten.de/podo/PointDefect -->

    <owl:Class rdf:about="http://purls.helmholtz-metadaten.de/podo/PointDefect">
        <rdfs:label>Point Defect</rdfs:label>
        <skos:definition>A point defect is a crystalline defect which is localized at or around a single lattice point. It is considered to be a zero-dimensional defect because it does not extend in any dimension in the lattice.</skos:definition>
    </owl:Class>
    


    <!-- http://purls.helmholtz-metadaten.de/podo/SchottkyDefect -->

    <owl:Class rdf:about="http://purls.helmholtz-metadaten.de/podo/SchottkyDefect">
        <rdfs:subClassOf rdf:resource="http://purls.helmholtz-metadaten.de/podo/PointDefect"/>
        <rdfs:label>Schottky Defect</rdfs:label>
        <skos:definition>A Schottky defect is a point defect which occurs in ionic crystals when oppositely charged ions create a vacancy in the interior of the lattice and go to the surface.</skos:definition>
    </owl:Class>
    


    <!-- http://purls.helmholtz-metadaten.de/podo/Self-interstitial -->

    <owl:Class rdf:about="http://purls.helmholtz-metadaten.de/podo/Self-interstitial">
        <rdfs:subClassOf rdf:resource="http://purls.helmholtz-metadaten.de/podo/Interstitial"/>
        <rdfs:label>Self-interstitial</rdfs:label>
        <skos:definition>A self-interstitial is an insterstitial defect where the atom occupying the interstitial site is of the same type as the matrix.</skos:definition>
    </owl:Class>
    


    <!-- http://purls.helmholtz-metadaten.de/podo/SubstitutionalImpurity -->

    <owl:Class rdf:about="http://purls.helmholtz-metadaten.de/podo/SubstitutionalImpurity">
        <rdfs:subClassOf rdf:resource="http://purls.helmholtz-metadaten.de/podo/Impurity"/>
        <rdfs:label>Substitutional Impurity</rdfs:label>
        <skos:definition>A substitutional impurity is an impurity where an atom of different type replaces a host or matrix atom.</skos:definition>
    </owl:Class>
    


    <!-- http://purls.helmholtz-metadaten.de/podo/Vacancy -->

    <owl:Class rdf:about="http://purls.helmholtz-metadaten.de/podo/Vacancy">
        <rdfs:subClassOf rdf:resource="http://purls.helmholtz-metadaten.de/podo/PointDefect"/>
        <rdfs:label>Vacancy</rdfs:label>
        <skos:definition>A vacancy is a point defect in which an atom is missing from its original lattice site.</skos:definition>
    </owl:Class>
    


    <!-- 
    ///////////////////////////////////////////////////////////////////////////////////////
    //
    // Annotations
    //
    ///////////////////////////////////////////////////////////////////////////////////////
     -->

    <rdf:Description rdf:about="http://www.w3.org/2004/02/skos/core#Collection">
        <skos:definition xml:lang="en">A meaningful collection of concepts.</skos:definition>
    </rdf:Description>
    <rdf:Description rdf:about="http://www.w3.org/2004/02/skos/core#Concept">
        <skos:definition xml:lang="en">An idea or notion; a unit of thought.</skos:definition>
    </rdf:Description>
    <rdf:Description rdf:about="http://www.w3.org/2004/02/skos/core#ConceptScheme">
        <skos:definition xml:lang="en">A set of concepts, optionally including statements about semantic relationships between those concepts.</skos:definition>
        <skos:example xml:lang="en">Thesauri, classification schemes, subject heading lists, taxonomies, &apos;folksonomies&apos;, and other types of controlled vocabulary are all examples of concept schemes. Concept schemes are also embedded in glossaries and terminologies.</skos:example>
    </rdf:Description>
    <rdf:Description rdf:about="http://www.w3.org/2004/02/skos/core#OrderedCollection">
        <skos:definition xml:lang="en">An ordered collection of concepts, where both the grouping and the ordering are meaningful.</skos:definition>
    </rdf:Description>
    <rdf:Description rdf:about="http://www.w3.org/2004/02/skos/core#broadMatch">
        <skos:definition xml:lang="en">skos:broadMatch is used to state a hierarchical mapping link between two conceptual resources in different concept schemes.</skos:definition>
    </rdf:Description>
    <rdf:Description rdf:about="http://www.w3.org/2004/02/skos/core#broader">
        <skos:definition xml:lang="en">Relates a concept to a concept that is more general in meaning.</skos:definition>
    </rdf:Description>
    <rdf:Description rdf:about="http://www.w3.org/2004/02/skos/core#broaderTransitive">
        <skos:definition>skos:broaderTransitive is a transitive superproperty of skos:broader.</skos:definition>
    </rdf:Description>
    <rdf:Description rdf:about="http://www.w3.org/2004/02/skos/core#changeNote">
        <skos:definition xml:lang="en">A note about a modification to a concept.</skos:definition>
    </rdf:Description>
    <rdf:Description rdf:about="http://www.w3.org/2004/02/skos/core#closeMatch">
        <skos:definition xml:lang="en">skos:closeMatch is used to link two concepts that are sufficiently similar that they can be used interchangeably in some information retrieval applications. In order to avoid the possibility of &quot;compound errors&quot; when combining mappings across more than two concept schemes, skos:closeMatch is not declared to be a transitive property.</skos:definition>
    </rdf:Description>
    <rdf:Description rdf:about="http://www.w3.org/2004/02/skos/core#editorialNote">
        <skos:definition xml:lang="en">A note for an editor, translator or maintainer of the vocabulary.</skos:definition>
    </rdf:Description>
    <rdf:Description rdf:about="http://www.w3.org/2004/02/skos/core#exactMatch">
        <skos:definition xml:lang="en">skos:exactMatch is used to link two concepts, indicating a high degree of confidence that the concepts can be used interchangeably across a wide range of information retrieval applications. skos:exactMatch is a transitive property, and is a sub-property of skos:closeMatch.</skos:definition>
    </rdf:Description>
    <rdf:Description rdf:about="http://www.w3.org/2004/02/skos/core#hasTopConcept">
        <skos:definition xml:lang="en">Relates, by convention, a concept scheme to a concept which is topmost in the broader/narrower concept hierarchies for that scheme, providing an entry point to these hierarchies.</skos:definition>
    </rdf:Description>
    <rdf:Description rdf:about="http://www.w3.org/2004/02/skos/core#hiddenLabel">
        <skos:definition xml:lang="en">A lexical label for a resource that should be hidden when generating visual displays of the resource, but should still be accessible to free text search operations.</skos:definition>
    </rdf:Description>
    <rdf:Description rdf:about="http://www.w3.org/2004/02/skos/core#historyNote">
        <skos:definition xml:lang="en">A note about the past state/use/meaning of a concept.</skos:definition>
    </rdf:Description>
    <rdf:Description rdf:about="http://www.w3.org/2004/02/skos/core#inScheme">
        <skos:definition xml:lang="en">Relates a resource (for example a concept) to a concept scheme in which it is included.</skos:definition>
    </rdf:Description>
    <rdf:Description rdf:about="http://www.w3.org/2004/02/skos/core#mappingRelation">
        <skos:definition xml:lang="en">Relates two concepts coming, by convention, from different schemes, and that have comparable meanings</skos:definition>
    </rdf:Description>
    <rdf:Description rdf:about="http://www.w3.org/2004/02/skos/core#member">
        <skos:definition xml:lang="en">Relates a collection to one of its members.</skos:definition>
    </rdf:Description>
    <rdf:Description rdf:about="http://www.w3.org/2004/02/skos/core#memberList">
        <skos:definition xml:lang="en">Relates an ordered collection to the RDF list containing its members.</skos:definition>
    </rdf:Description>
    <rdf:Description rdf:about="http://www.w3.org/2004/02/skos/core#narrowMatch">
        <skos:definition xml:lang="en">skos:narrowMatch is used to state a hierarchical mapping link between two conceptual resources in different concept schemes.</skos:definition>
    </rdf:Description>
    <rdf:Description rdf:about="http://www.w3.org/2004/02/skos/core#narrower">
        <skos:definition xml:lang="en">Relates a concept to a concept that is more specific in meaning.</skos:definition>
    </rdf:Description>
    <rdf:Description rdf:about="http://www.w3.org/2004/02/skos/core#narrowerTransitive">
        <skos:definition>skos:narrowerTransitive is a transitive superproperty of skos:narrower.</skos:definition>
    </rdf:Description>
    <rdf:Description rdf:about="http://www.w3.org/2004/02/skos/core#notation">
        <skos:definition xml:lang="en">A notation, also known as classification code, is a string of characters such as &quot;T58.5&quot; or &quot;303.4833&quot; used to uniquely identify a concept within the scope of a given concept scheme.</skos:definition>
    </rdf:Description>
    <rdf:Description rdf:about="http://www.w3.org/2004/02/skos/core#related">
        <skos:definition xml:lang="en">Relates a concept to a concept with which there is an associative semantic relationship.</skos:definition>
    </rdf:Description>
    <rdf:Description rdf:about="http://www.w3.org/2004/02/skos/core#relatedMatch">
        <skos:definition xml:lang="en">skos:relatedMatch is used to state an associative mapping link between two conceptual resources in different concept schemes.</skos:definition>
    </rdf:Description>
    <rdf:Description rdf:about="http://www.w3.org/2004/02/skos/core#scopeNote">
        <skos:definition xml:lang="en">A note that helps to clarify the meaning and/or the use of a concept.</skos:definition>
    </rdf:Description>
    <rdf:Description rdf:about="http://www.w3.org/2004/02/skos/core#semanticRelation">
        <skos:definition xml:lang="en">Links a concept to a concept related by meaning.</skos:definition>
    </rdf:Description>
    <rdf:Description rdf:about="http://www.w3.org/2004/02/skos/core#topConceptOf">
        <skos:definition xml:lang="en">Relates a concept to the concept scheme that it is a top level concept of.</skos:definition>
    </rdf:Description>
</rdf:RDF>



<!-- Generated by the OWL API (version 4.5.9.2019-02-01T07:24:44Z) https://github.com/owlcs/owlapi -->

