<?xml version="1.0"?>
<rdf:RDF xmlns="http://purls.helmholtz-metadaten.de/pldo/"
     xml:base="http://purls.helmholtz-metadaten.de/pldo/"
     xmlns:dc="http://purl.org/dc/elements/1.1/"
     xmlns:owl="http://www.w3.org/2002/07/owl#"
     xmlns:rdf="http://www.w3.org/1999/02/22-rdf-syntax-ns#"
     xmlns:xml="http://www.w3.org/XML/1998/namespace"
     xmlns:xsd="http://www.w3.org/2001/XMLSchema#"
     xmlns:rdfs="http://www.w3.org/2000/01/rdf-schema#"
     xmlns:skos="http://www.w3.org/2004/02/skos/core#"
     xmlns:terms="http://purl.org/dc/terms/">
    <owl:Ontology rdf:about="http://purls.helmholtz-metadaten.de/pldo/">
        <terms:contributor>https://orcid.org/0000-0001-9560-4728</terms:contributor>
        <terms:contributor>https://orcid.org/0000-0002-5149-603X</terms:contributor>
        <terms:contributor>https://orcid.org/0000-0002-6776-1213</terms:contributor>
        <terms:contributor>https://orcid.org/0000-0003-0698-4891</terms:contributor>
        <terms:creator>https://orcid.org/0000-0001-7564-7990</terms:creator>
        <terms:description>PLDO focuses on the description of planar defects in crystalline materials.</terms:description>
        <terms:title>Planar Defects Ontology (PLDO)</terms:title>
    </owl:Ontology>
    


    <!-- 
    ///////////////////////////////////////////////////////////////////////////////////////
    //
    // Annotation properties
    //
    ///////////////////////////////////////////////////////////////////////////////////////
     -->

    


    <!-- http://purl.org/dc/elements/1.1/contributor -->

    <owl:AnnotationProperty rdf:about="http://purl.org/dc/elements/1.1/contributor"/>
    


    <!-- http://purl.org/dc/elements/1.1/creator -->

    <owl:AnnotationProperty rdf:about="http://purl.org/dc/elements/1.1/creator"/>
    


    <!-- http://purl.org/dc/elements/1.1/description -->

    <owl:AnnotationProperty rdf:about="http://purl.org/dc/elements/1.1/description"/>
    


    <!-- http://purl.org/dc/elements/1.1/title -->

    <owl:AnnotationProperty rdf:about="http://purl.org/dc/elements/1.1/title"/>
    


    <!-- http://purl.org/dc/terms/abstract -->

    <owl:AnnotationProperty rdf:about="http://purl.org/dc/terms/abstract">
        <rdfs:subPropertyOf rdf:resource="http://purl.org/dc/terms/description"/>
    </owl:AnnotationProperty>
    


    <!-- http://purl.org/dc/terms/alternative -->

    <owl:AnnotationProperty rdf:about="http://purl.org/dc/terms/alternative">
        <rdfs:subPropertyOf rdf:resource="http://purl.org/dc/terms/title"/>
    </owl:AnnotationProperty>
    


    <!-- http://purl.org/dc/terms/contributor -->

    <owl:AnnotationProperty rdf:about="http://purl.org/dc/terms/contributor">
        <rdfs:comment xml:lang="en-us">Examples of a Contributor include a person, an organization, or a service. Typically, the name of a Contributor should be used to indicate the entity.</rdfs:comment>
        <rdfs:label xml:lang="en-us">Contributor</rdfs:label>
        <skos:definition xml:lang="en-us">An entity responsible for making contributions to the resource.</skos:definition>
        <rdfs:subPropertyOf rdf:resource="http://purl.org/dc/elements/1.1/contributor"/>
        <rdfs:range rdf:resource="http://purl.org/dc/terms/Agent"/>
    </owl:AnnotationProperty>
    


    <!-- http://purl.org/dc/terms/creator -->

    <owl:AnnotationProperty rdf:about="http://purl.org/dc/terms/creator">
        <rdfs:comment xml:lang="en-us">Examples of a Creator include a person, an organization, or a service. Typically, the name of a Creator should be used to indicate the entity.</rdfs:comment>
        <rdfs:label xml:lang="en-us">Creator</rdfs:label>
        <skos:definition xml:lang="en-us">An entity primarily responsible for making the resource.</skos:definition>
        <rdfs:subPropertyOf rdf:resource="http://purl.org/dc/elements/1.1/creator"/>
        <rdfs:subPropertyOf rdf:resource="http://purl.org/dc/terms/contributor"/>
        <rdfs:range rdf:resource="http://purl.org/dc/terms/Agent"/>
    </owl:AnnotationProperty>
    


    <!-- http://purl.org/dc/terms/description -->

    <owl:AnnotationProperty rdf:about="http://purl.org/dc/terms/description">
        <rdfs:comment xml:lang="en-us">Description may include but is not limited to: an abstract, a table of contents, a graphical representation, or a free-text account of the resource.</rdfs:comment>
        <rdfs:label xml:lang="en-us">Description</rdfs:label>
        <skos:definition xml:lang="en-us">An account of the resource.</skos:definition>
        <rdfs:subPropertyOf rdf:resource="http://purl.org/dc/elements/1.1/description"/>
    </owl:AnnotationProperty>
    


    <!-- http://purl.org/dc/terms/tableOfContents -->

    <owl:AnnotationProperty rdf:about="http://purl.org/dc/terms/tableOfContents">
        <rdfs:subPropertyOf rdf:resource="http://purl.org/dc/terms/description"/>
    </owl:AnnotationProperty>
    


    <!-- http://purl.org/dc/terms/title -->

    <owl:AnnotationProperty rdf:about="http://purl.org/dc/terms/title">
        <rdfs:label xml:lang="en-us">Title</rdfs:label>
        <skos:definition xml:lang="en-us">A name given to the resource.</skos:definition>
        <skos:note xml:lang="en-us">In current practice, this term is used primarily with literal values; however, there are important uses with non-literal values as well. As of December 2007, the DCMI Usage Board is leaving this range unspecified pending an investigation of options.</skos:note>
        <rdfs:subPropertyOf rdf:resource="http://purl.org/dc/elements/1.1/title"/>
    </owl:AnnotationProperty>
    


    <!-- http://www.w3.org/2004/02/skos/core#altLabel -->

    <owl:AnnotationProperty rdf:about="http://www.w3.org/2004/02/skos/core#altLabel">
        <rdfs:comment xml:lang="en">The range of skos:altLabel is the class of RDF plain literals.</rdfs:comment>
        <rdfs:comment xml:lang="en">skos:prefLabel, skos:altLabel and skos:hiddenLabel are pairwise disjoint properties.</rdfs:comment>
        <rdfs:isDefinedBy rdf:resource="http://www.w3.org/2004/02/skos/core"/>
        <rdfs:label xml:lang="en">alternative label</rdfs:label>
        <skos:definition xml:lang="en">An alternative lexical label for a resource.</skos:definition>
        <skos:example xml:lang="en">Acronyms, abbreviations, spelling variants, and irregular plural/singular forms may be included among the alternative labels for a concept. Mis-spelled terms are normally included as hidden labels (see skos:hiddenLabel).</skos:example>
        <rdfs:subPropertyOf rdf:resource="http://www.w3.org/2000/01/rdf-schema#label"/>
    </owl:AnnotationProperty>
    


    <!-- http://www.w3.org/2004/02/skos/core#definition -->

    <owl:AnnotationProperty rdf:about="http://www.w3.org/2004/02/skos/core#definition">
        <rdfs:isDefinedBy rdf:resource="http://www.w3.org/2004/02/skos/core"/>
        <rdfs:label xml:lang="en">definition</rdfs:label>
        <skos:definition xml:lang="en">A statement or formal explanation of the meaning of a concept.</skos:definition>
        <rdfs:subPropertyOf rdf:resource="http://www.w3.org/2004/02/skos/core#note"/>
    </owl:AnnotationProperty>
    


    <!-- http://www.w3.org/2004/02/skos/core#example -->

    <owl:AnnotationProperty rdf:about="http://www.w3.org/2004/02/skos/core#example">
        <rdfs:isDefinedBy rdf:resource="http://www.w3.org/2004/02/skos/core"/>
        <rdfs:label xml:lang="en">example</rdfs:label>
        <skos:definition xml:lang="en">An example of the use of a concept.</skos:definition>
        <rdfs:subPropertyOf rdf:resource="http://www.w3.org/2004/02/skos/core#note"/>
    </owl:AnnotationProperty>
    


    <!-- http://www.w3.org/2004/02/skos/core#note -->

    <owl:AnnotationProperty rdf:about="http://www.w3.org/2004/02/skos/core#note">
        <skos:definition xml:lang="en">A general note, for any purpose.</skos:definition>
    </owl:AnnotationProperty>
    


    <!-- http://www.w3.org/2004/02/skos/core#prefLabel -->

    <owl:AnnotationProperty rdf:about="http://www.w3.org/2004/02/skos/core#prefLabel">
        <rdfs:comment xml:lang="en">A resource has no more than one value of skos:prefLabel per language tag, and no more than one value of skos:prefLabel without language tag.</rdfs:comment>
        <rdfs:comment xml:lang="en">The range of skos:prefLabel is the class of RDF plain literals.</rdfs:comment>
        <rdfs:comment xml:lang="en">skos:prefLabel, skos:altLabel and skos:hiddenLabel are pairwise
      disjoint properties.</rdfs:comment>
        <rdfs:isDefinedBy rdf:resource="http://www.w3.org/2004/02/skos/core"/>
        <rdfs:label xml:lang="en">preferred label</rdfs:label>
        <skos:definition xml:lang="en">The preferred lexical label for a resource, in a given language.</skos:definition>
        <rdfs:subPropertyOf rdf:resource="http://www.w3.org/2000/01/rdf-schema#label"/>
    </owl:AnnotationProperty>
    


    <!-- 
    ///////////////////////////////////////////////////////////////////////////////////////
    //
    // Object Properties
    //
    ///////////////////////////////////////////////////////////////////////////////////////
     -->

    


    <!-- http://purls.helmholtz-metadaten.de/pldo/hasTiltComponent -->

    <owl:ObjectProperty rdf:about="http://purls.helmholtz-metadaten.de/pldo/hasTiltComponent">
        <rdfs:domain rdf:resource="http://purls.helmholtz-metadaten.de/pldo/MixedGrainBoundary"/>
        <rdfs:range rdf:resource="http://purls.helmholtz-metadaten.de/pldo/TiltGrainBoundary"/>
        <rdfs:label>has tilt component</rdfs:label>
        <skos:definition>The relation between a mixed grain boundary and the tilt grain boundary component.</skos:definition>
    </owl:ObjectProperty>
    


    <!-- http://purls.helmholtz-metadaten.de/pldo/hasTwistComponent -->

    <owl:ObjectProperty rdf:about="http://purls.helmholtz-metadaten.de/pldo/hasTwistComponent">
        <rdfs:domain rdf:resource="http://purls.helmholtz-metadaten.de/pldo/MixedGrainBoundary"/>
        <rdfs:range rdf:resource="http://purls.helmholtz-metadaten.de/pldo/TwistGrainBoundary"/>
        <rdfs:label>has twist component</rdfs:label>
        <skos:definition>The relation between a mixed grain boundary and the twist grain boundary component.</skos:definition>
    </owl:ObjectProperty>
    


    <!-- 
    ///////////////////////////////////////////////////////////////////////////////////////
    //
    // Data properties
    //
    ///////////////////////////////////////////////////////////////////////////////////////
     -->

    


    <!-- http://purls.helmholtz-metadaten.de/pldo/geometricalDegreesOfFreedom -->

    <owl:DatatypeProperty rdf:about="http://purls.helmholtz-metadaten.de/pldo/geometricalDegreesOfFreedom">
        <rdfs:domain rdf:resource="http://purls.helmholtz-metadaten.de/pldo/GrainBoundary"/>
        <rdfs:label>geometrical degrees of freedom</rdfs:label>
        <skos:definition>The geometrical degrees of freedom are the parameters that are necessary to characterize a grain boundary.</skos:definition>
    </owl:DatatypeProperty>
    


    <!-- http://purls.helmholtz-metadaten.de/pldo/hasGBplane -->

    <owl:DatatypeProperty rdf:about="http://purls.helmholtz-metadaten.de/pldo/hasGBplane">
        <rdfs:subPropertyOf rdf:resource="http://purls.helmholtz-metadaten.de/pldo/macroscopicDegreesOfFreedom"/>
        <rdfs:domain rdf:resource="http://purls.helmholtz-metadaten.de/pldo/GrainBoundary"/>
        <rdfs:range rdf:resource="http://www.w3.org/2001/XMLSchema#string"/>
        <rdfs:label>has GB plane</rdfs:label>
        <skos:definition>A data property indicating the grain boundary (GB) plane using Miller Indices.</skos:definition>
    </owl:DatatypeProperty>
    


    <!-- http://purls.helmholtz-metadaten.de/pldo/hasMisorientationAngle -->

    <owl:DatatypeProperty rdf:about="http://purls.helmholtz-metadaten.de/pldo/hasMisorientationAngle">
        <rdfs:subPropertyOf rdf:resource="http://purls.helmholtz-metadaten.de/pldo/macroscopicDegreesOfFreedom"/>
        <rdfs:domain rdf:resource="http://purls.helmholtz-metadaten.de/pldo/GrainBoundary"/>
        <rdfs:range rdf:resource="http://www.w3.org/2001/XMLSchema#float"/>
        <rdfs:label>has misorientation angle</rdfs:label>
        <skos:definition>A data property indicating the misorientation angle (θ) of the grains with respect to each other.</skos:definition>
    </owl:DatatypeProperty>
    


    <!-- http://purls.helmholtz-metadaten.de/pldo/hasRotationAxis -->

    <owl:DatatypeProperty rdf:about="http://purls.helmholtz-metadaten.de/pldo/hasRotationAxis">
        <rdfs:subPropertyOf rdf:resource="http://purls.helmholtz-metadaten.de/pldo/macroscopicDegreesOfFreedom"/>
        <rdfs:domain rdf:resource="http://purls.helmholtz-metadaten.de/pldo/GrainBoundary"/>
        <rdfs:range rdf:resource="http://www.w3.org/2001/XMLSchema#string"/>
        <rdfs:label>has rotation axis</rdfs:label>
        <skos:definition>A data property indication the rotation axis [uvw].</skos:definition>
    </owl:DatatypeProperty>
    


    <!-- http://purls.helmholtz-metadaten.de/pldo/hasSigmaValue -->

    <owl:DatatypeProperty rdf:about="http://purls.helmholtz-metadaten.de/pldo/hasSigmaValue">
        <rdfs:domain rdf:resource="http://purls.helmholtz-metadaten.de/pldo/GrainBoundary"/>
        <rdfs:range rdf:resource="http://www.w3.org/2001/XMLSchema#integer"/>
        <rdfs:comment>Sigma value of a GB is the coincidence index, calculated as the coincidence unit cell volume by the crystal primitive unit cell volume. The coincidence index refers to the Coincidence Site Lattice (CSL).</rdfs:comment>
        <rdfs:label>has sigma value</rdfs:label>
        <skos:definition>A data property linking a GB with its sigma value.</skos:definition>
    </owl:DatatypeProperty>
    


    <!-- http://purls.helmholtz-metadaten.de/pldo/macroscopicDegreesOfFreedom -->

    <owl:DatatypeProperty rdf:about="http://purls.helmholtz-metadaten.de/pldo/macroscopicDegreesOfFreedom">
        <rdfs:subPropertyOf rdf:resource="http://purls.helmholtz-metadaten.de/pldo/geometricalDegreesOfFreedom"/>
        <rdfs:domain rdf:resource="http://purls.helmholtz-metadaten.de/pldo/GrainBoundary"/>
        <rdfs:comment>In simulations of grain boundaries, the macroscopic DOFs are imposed on the structure.</rdfs:comment>
        <rdfs:label>macroscopic degrees of freedom</rdfs:label>
        <skos:definition>There are five macroscopic degrees of freedom (DOFs) that are sufficient to describe the thermodynamic description of the grain boundary.</skos:definition>
    </owl:DatatypeProperty>
    


    <!-- http://purls.helmholtz-metadaten.de/pldo/microscopicDegreesOfFreedom -->

    <owl:DatatypeProperty rdf:about="http://purls.helmholtz-metadaten.de/pldo/microscopicDegreesOfFreedom">
        <rdfs:subPropertyOf rdf:resource="http://purls.helmholtz-metadaten.de/pldo/geometricalDegreesOfFreedom"/>
        <rdfs:domain rdf:resource="http://purls.helmholtz-metadaten.de/pldo/GrainBoundary"/>
        <rdfs:comment>In simulations of grain boundaries, the microscopic DOFs are obtained after the grain boundary energy minimization.</rdfs:comment>
        <rdfs:label>microscopic degrees of freedom</rdfs:label>
        <skos:definition>The microscopic degrees of freedom (DOFs) refer to the translation of one crystal with respect to the other at the microscopic scale. The microscopic parameters result from the relaxation process and are not independent of the macroscopic parameters.</skos:definition>
    </owl:DatatypeProperty>
    


    <!-- 
    ///////////////////////////////////////////////////////////////////////////////////////
    //
    // Classes
    //
    ///////////////////////////////////////////////////////////////////////////////////////
     -->

    


    <!-- http://purls.helmholtz-metadaten.de/pldo/AntiphaseBoundary -->

    <owl:Class rdf:about="http://purls.helmholtz-metadaten.de/pldo/AntiphaseBoundary">
        <rdfs:subClassOf rdf:resource="http://purls.helmholtz-metadaten.de/pldo/PlanarDefect"/>
        <rdfs:label>Antiphase Boundary</rdfs:label>
        <skos:altLabel>APB</skos:altLabel>
        <skos:definition>An antiphase boundary is a planar defect which occurs in ordered alloys. The boundary separates two domains of the same ordered phase.</skos:definition>
    </owl:Class>
    


    <!-- http://purls.helmholtz-metadaten.de/pldo/GrainBoundary -->

    <owl:Class rdf:about="http://purls.helmholtz-metadaten.de/pldo/GrainBoundary">
        <rdfs:subClassOf rdf:resource="http://purls.helmholtz-metadaten.de/pldo/PlanarDefect"/>
        <rdfs:label>Grain Boundary</rdfs:label>
        <skos:altLabel>GB</skos:altLabel>
        <skos:definition>A grain boundary is a planar defect that separates two crystals (or grains) of the same material.</skos:definition>
    </owl:Class>
    


    <!-- http://purls.helmholtz-metadaten.de/pldo/LowAngleGrainBoundary -->

    <owl:Class rdf:about="http://purls.helmholtz-metadaten.de/pldo/LowAngleGrainBoundary">
        <rdfs:subClassOf rdf:resource="http://purls.helmholtz-metadaten.de/pldo/GrainBoundary"/>
        <rdfs:comment>Reference: ISBN 978-94-007-4968-9</rdfs:comment>
        <rdfs:label>Low Angle Grain Boundary</rdfs:label>
        <skos:altLabel>Low-Angle Grain Boundary</skos:altLabel>
        <skos:definition>A low angle GB is a grain boundary with a misorientation angle lower than 15 degrees.</skos:definition>
    </owl:Class>
    


    <!-- http://purls.helmholtz-metadaten.de/pldo/MixedGrainBoundary -->

    <owl:Class rdf:about="http://purls.helmholtz-metadaten.de/pldo/MixedGrainBoundary">
        <rdfs:subClassOf rdf:resource="http://purls.helmholtz-metadaten.de/pldo/GrainBoundary"/>
        <rdfs:comment>Reference: ISBN 978-94-007-4968-9</rdfs:comment>
        <rdfs:label>Mixed Grain Boundary</rdfs:label>
        <skos:definition>A mixed grain boundary is a grain boundary where the [uvw] rotation axis has perpendicular and parallel components with respect to the boundary plane.</skos:definition>
    </owl:Class>
    


    <!-- http://purls.helmholtz-metadaten.de/pldo/PlanarDefect -->

    <owl:Class rdf:about="http://purls.helmholtz-metadaten.de/pldo/PlanarDefect">
        <rdfs:label>Planar Defect</rdfs:label>
        <skos:altLabel>Interface</skos:altLabel>
        <skos:definition>A planar defect is a defect of the crystal structure across a plane. It is considered to be a two-dimensional defect, such as an internal interface or the surface.</skos:definition>
    </owl:Class>
    


    <!-- http://purls.helmholtz-metadaten.de/pldo/StackingFault -->

    <owl:Class rdf:about="http://purls.helmholtz-metadaten.de/pldo/StackingFault">
        <rdfs:subClassOf rdf:resource="http://purls.helmholtz-metadaten.de/pldo/PlanarDefect"/>
        <rdfs:label>Stacking Fault</rdfs:label>
        <skos:definition>A stacking fault is a planar defect created by an error (fault) in the order of the sequential layering of crystallographic planes.</skos:definition>
    </owl:Class>
    


    <!-- http://purls.helmholtz-metadaten.de/pldo/Surface -->

    <owl:Class rdf:about="http://purls.helmholtz-metadaten.de/pldo/Surface">
        <rdfs:subClassOf rdf:resource="http://purls.helmholtz-metadaten.de/pldo/PlanarDefect"/>
        <rdfs:label>Surface</rdfs:label>
        <skos:definition>The free surface (or external surface) of the material is a planar defect where the surface atoms have no neighbours or cohesive bonds on the external side.</skos:definition>
    </owl:Class>
    


    <!-- http://purls.helmholtz-metadaten.de/pldo/SymmetricalTiltGrainBoundary -->

    <owl:Class rdf:about="http://purls.helmholtz-metadaten.de/pldo/SymmetricalTiltGrainBoundary">
        <rdfs:subClassOf rdf:resource="http://purls.helmholtz-metadaten.de/pldo/TiltGrainBoundary"/>
        <rdfs:comment>Reference: ISBN 978-94-007-4968-9</rdfs:comment>
        <rdfs:label>Symmetrical Tilt Grain Boundary</rdfs:label>
        <skos:definition>A symmetrical tilt grain boundary is a tilt grain boundary where the two grains are symmetric. The boundary plane has the same Miller indices in crystals I and II: {hkl}_1 = {hkl}_2.</skos:definition>
    </owl:Class>
    


    <!-- http://purls.helmholtz-metadaten.de/pldo/TiltGrainBoundary -->

    <owl:Class rdf:about="http://purls.helmholtz-metadaten.de/pldo/TiltGrainBoundary">
        <rdfs:subClassOf rdf:resource="http://purls.helmholtz-metadaten.de/pldo/GrainBoundary"/>
        <rdfs:comment>Reference: ISBN 978-94-007-4968-9</rdfs:comment>
        <rdfs:label>Tilt Grain Boundary</rdfs:label>
        <skos:altLabel>Tilt Boundary</skos:altLabel>
        <skos:definition>A twist boundary is a grain boundary with a [uvw] rotation axis perpendicular to the boundary plane.</skos:definition>
    </owl:Class>
    


    <!-- http://purls.helmholtz-metadaten.de/pldo/TwinBoundary -->

    <owl:Class rdf:about="http://purls.helmholtz-metadaten.de/pldo/TwinBoundary">
        <rdfs:subClassOf rdf:resource="http://purls.helmholtz-metadaten.de/pldo/PlanarDefect"/>
        <rdfs:label>Twin Boundary</rdfs:label>
        <skos:definition>A twin boundary is a planar defect that occurs between two separate crystals which are mirror images of each other, both crystals should have the same crystal structure.</skos:definition>
    </owl:Class>
    


    <!-- http://purls.helmholtz-metadaten.de/pldo/TwistGrainBoundary -->

    <owl:Class rdf:about="http://purls.helmholtz-metadaten.de/pldo/TwistGrainBoundary">
        <rdfs:subClassOf rdf:resource="http://purls.helmholtz-metadaten.de/pldo/GrainBoundary"/>
        <rdfs:comment>Reference: ISBN 978-94-007-4968-9</rdfs:comment>
        <rdfs:label>Twist Grain Boundary</rdfs:label>
        <skos:altLabel>Twist Boundary</skos:altLabel>
        <skos:definition>A twist boundary is a grain boundary with a [uvw] rotation axis contained within the boundary plane.</skos:definition>
    </owl:Class>
    


    <!-- 
    ///////////////////////////////////////////////////////////////////////////////////////
    //
    // Annotations
    //
    ///////////////////////////////////////////////////////////////////////////////////////
     -->

    <rdf:Description rdf:about="http://www.w3.org/2004/02/skos/core#Collection">
        <skos:definition xml:lang="en">A meaningful collection of concepts.</skos:definition>
    </rdf:Description>
    <rdf:Description rdf:about="http://www.w3.org/2004/02/skos/core#Concept">
        <skos:definition xml:lang="en">An idea or notion; a unit of thought.</skos:definition>
    </rdf:Description>
    <rdf:Description rdf:about="http://www.w3.org/2004/02/skos/core#ConceptScheme">
        <skos:definition xml:lang="en">A set of concepts, optionally including statements about semantic relationships between those concepts.</skos:definition>
        <skos:example xml:lang="en">Thesauri, classification schemes, subject heading lists, taxonomies, &apos;folksonomies&apos;, and other types of controlled vocabulary are all examples of concept schemes. Concept schemes are also embedded in glossaries and terminologies.</skos:example>
    </rdf:Description>
    <rdf:Description rdf:about="http://www.w3.org/2004/02/skos/core#OrderedCollection">
        <skos:definition xml:lang="en">An ordered collection of concepts, where both the grouping and the ordering are meaningful.</skos:definition>
    </rdf:Description>
    <rdf:Description rdf:about="http://www.w3.org/2004/02/skos/core#broadMatch">
        <skos:definition xml:lang="en">skos:broadMatch is used to state a hierarchical mapping link between two conceptual resources in different concept schemes.</skos:definition>
    </rdf:Description>
    <rdf:Description rdf:about="http://www.w3.org/2004/02/skos/core#broader">
        <skos:definition xml:lang="en">Relates a concept to a concept that is more general in meaning.</skos:definition>
    </rdf:Description>
    <rdf:Description rdf:about="http://www.w3.org/2004/02/skos/core#broaderTransitive">
        <skos:definition>skos:broaderTransitive is a transitive superproperty of skos:broader.</skos:definition>
    </rdf:Description>
    <rdf:Description rdf:about="http://www.w3.org/2004/02/skos/core#changeNote">
        <skos:definition xml:lang="en">A note about a modification to a concept.</skos:definition>
    </rdf:Description>
    <rdf:Description rdf:about="http://www.w3.org/2004/02/skos/core#closeMatch">
        <skos:definition xml:lang="en">skos:closeMatch is used to link two concepts that are sufficiently similar that they can be used interchangeably in some information retrieval applications. In order to avoid the possibility of &quot;compound errors&quot; when combining mappings across more than two concept schemes, skos:closeMatch is not declared to be a transitive property.</skos:definition>
    </rdf:Description>
    <rdf:Description rdf:about="http://www.w3.org/2004/02/skos/core#editorialNote">
        <skos:definition xml:lang="en">A note for an editor, translator or maintainer of the vocabulary.</skos:definition>
    </rdf:Description>
    <rdf:Description rdf:about="http://www.w3.org/2004/02/skos/core#exactMatch">
        <skos:definition xml:lang="en">skos:exactMatch is used to link two concepts, indicating a high degree of confidence that the concepts can be used interchangeably across a wide range of information retrieval applications. skos:exactMatch is a transitive property, and is a sub-property of skos:closeMatch.</skos:definition>
    </rdf:Description>
    <rdf:Description rdf:about="http://www.w3.org/2004/02/skos/core#hasTopConcept">
        <skos:definition xml:lang="en">Relates, by convention, a concept scheme to a concept which is topmost in the broader/narrower concept hierarchies for that scheme, providing an entry point to these hierarchies.</skos:definition>
    </rdf:Description>
    <rdf:Description rdf:about="http://www.w3.org/2004/02/skos/core#hiddenLabel">
        <skos:definition xml:lang="en">A lexical label for a resource that should be hidden when generating visual displays of the resource, but should still be accessible to free text search operations.</skos:definition>
    </rdf:Description>
    <rdf:Description rdf:about="http://www.w3.org/2004/02/skos/core#historyNote">
        <skos:definition xml:lang="en">A note about the past state/use/meaning of a concept.</skos:definition>
    </rdf:Description>
    <rdf:Description rdf:about="http://www.w3.org/2004/02/skos/core#inScheme">
        <skos:definition xml:lang="en">Relates a resource (for example a concept) to a concept scheme in which it is included.</skos:definition>
    </rdf:Description>
    <rdf:Description rdf:about="http://www.w3.org/2004/02/skos/core#mappingRelation">
        <skos:definition xml:lang="en">Relates two concepts coming, by convention, from different schemes, and that have comparable meanings</skos:definition>
    </rdf:Description>
    <rdf:Description rdf:about="http://www.w3.org/2004/02/skos/core#member">
        <skos:definition xml:lang="en">Relates a collection to one of its members.</skos:definition>
    </rdf:Description>
    <rdf:Description rdf:about="http://www.w3.org/2004/02/skos/core#memberList">
        <skos:definition xml:lang="en">Relates an ordered collection to the RDF list containing its members.</skos:definition>
    </rdf:Description>
    <rdf:Description rdf:about="http://www.w3.org/2004/02/skos/core#narrowMatch">
        <skos:definition xml:lang="en">skos:narrowMatch is used to state a hierarchical mapping link between two conceptual resources in different concept schemes.</skos:definition>
    </rdf:Description>
    <rdf:Description rdf:about="http://www.w3.org/2004/02/skos/core#narrower">
        <skos:definition xml:lang="en">Relates a concept to a concept that is more specific in meaning.</skos:definition>
    </rdf:Description>
    <rdf:Description rdf:about="http://www.w3.org/2004/02/skos/core#narrowerTransitive">
        <skos:definition>skos:narrowerTransitive is a transitive superproperty of skos:narrower.</skos:definition>
    </rdf:Description>
    <rdf:Description rdf:about="http://www.w3.org/2004/02/skos/core#notation">
        <skos:definition xml:lang="en">A notation, also known as classification code, is a string of characters such as &quot;T58.5&quot; or &quot;303.4833&quot; used to uniquely identify a concept within the scope of a given concept scheme.</skos:definition>
    </rdf:Description>
    <rdf:Description rdf:about="http://www.w3.org/2004/02/skos/core#related">
        <skos:definition xml:lang="en">Relates a concept to a concept with which there is an associative semantic relationship.</skos:definition>
    </rdf:Description>
    <rdf:Description rdf:about="http://www.w3.org/2004/02/skos/core#relatedMatch">
        <skos:definition xml:lang="en">skos:relatedMatch is used to state an associative mapping link between two conceptual resources in different concept schemes.</skos:definition>
    </rdf:Description>
    <rdf:Description rdf:about="http://www.w3.org/2004/02/skos/core#scopeNote">
        <skos:definition xml:lang="en">A note that helps to clarify the meaning and/or the use of a concept.</skos:definition>
    </rdf:Description>
    <rdf:Description rdf:about="http://www.w3.org/2004/02/skos/core#semanticRelation">
        <skos:definition xml:lang="en">Links a concept to a concept related by meaning.</skos:definition>
    </rdf:Description>
    <rdf:Description rdf:about="http://www.w3.org/2004/02/skos/core#topConceptOf">
        <skos:definition xml:lang="en">Relates a concept to the concept scheme that it is a top level concept of.</skos:definition>
    </rdf:Description>
</rdf:RDF>



<!-- Generated by the OWL API (version 4.5.9.2019-02-01T07:24:44Z) https://github.com/owlcs/owlapi -->

